Refactor half of fp_red

theories/fp_red.v
@@ -8,7 +8,7 @@ Require Import Arith.Wf_nat (well_founded_lt_compat).
 Require Import Psatz.
 From stdpp Require Import relations (rtc (..), rtc_once, rtc_r, sn).
 From Hammer Require Import Tactics.
-Require Import Autosubst2.core Autosubst2.fintype Autosubst2.syntax common.
+Require Import Autosubst2.core Autosubst2.unscoped Autosubst2.syntax common.
 Require Import Btauto.
 Require Import Cdcl.Itauto.
 
@@ -23,7 +23,7 @@ Ltac2 spec_refl () :=
 Ltac spec_refl := ltac2:(Control.enter spec_refl).
 
 Module EPar.
-  Inductive R {n} : PTm n -> PTm n ->  Prop :=
+  Inductive R : PTm -> PTm ->  Prop :=
   (****************** Eta ***********************)
   | AppEta a0 a1 :
     R a0 a1 ->
@@ -54,8 +54,6 @@ Module EPar.
     R A0 A1 ->
     R B0 B1 ->
     R (PBind p A0 B0) (PBind p A1 B1)
-  | BotCong :
-    R PBot PBot
   | NatCong :
     R PNat PNat
   | IndCong P0 P1 a0 a1 b0 b1 c0 c1 :
@@ -72,64 +70,64 @@ Module EPar.
     (* ------------ *)
     R (PSuc a0) (PSuc a1).
 
-  Lemma refl n (a : PTm n) : R a a.
+  Lemma refl (a : PTm) : R a a.
   Proof.
-    elim : n / a; hauto lq:on ctrs:R.
+    elim : a; hauto lq:on ctrs:R.
   Qed.
 
-  Derive Dependent Inversion inv with (forall n (a b : PTm n), R a b) Sort Prop.
+  Derive Dependent Inversion inv with (forall (a b : PTm), R a b) Sort Prop.
 
-  Lemma AppEta' n a0 a1 (u : PTm n) :
+  Lemma AppEta' a0 a1 (u : PTm) :
     u = (PAbs (PApp (ren_PTm shift a0) (VarPTm var_zero))) ->
     R a0 a1 ->
     R u a1.
   Proof. move => ->. apply AppEta. Qed.
 
-  Lemma renaming n m (a b : PTm n) (ξ : fin n -> fin m) :
+  Lemma renaming (a b : PTm) (ξ : nat -> nat) :
     R a b -> R (ren_PTm ξ a) (ren_PTm ξ b).
   Proof.
-    move => h. move : m ξ.
-    elim : n a b /h.
+    move => h. move : ξ.
+    elim : a b /h.
 
     all : try qauto ctrs:R.
 
-    move => n a0 a1 ha iha m ξ /=.
+    move => a0 a1 ha iha ξ /=.
     eapply AppEta'; eauto. by asimpl.
   Qed.
 
-  Lemma morphing_ren n m p (ρ0 ρ1 : fin n -> PTm m) (ξ : fin m -> fin p) :
+  Lemma morphing_ren (ρ0 ρ1 : nat -> PTm) (ξ : nat -> nat) :
     (forall i, R (ρ0 i) (ρ1 i)) ->
-    (forall i, R ((funcomp (ren_PTm ξ) ρ0) i) ((funcomp (ren_PTm ξ) ρ1) i)).
+    (forall i, R (funcomp (ren_PTm ξ) ρ0 i) ((funcomp (ren_PTm ξ) ρ1) i)).
   Proof. eauto using renaming. Qed.
 
-  Lemma morphing_ext n m (ρ0 ρ1 : fin n -> PTm m) a b  :
+  Lemma morphing_ext (ρ0 ρ1 : nat -> PTm) a b  :
     R a b ->
     (forall i, R (ρ0 i) (ρ1 i)) ->
     (forall i, R ((scons a ρ0) i) ((scons b ρ1) i)).
-  Proof. hauto q:on inv:option. Qed.
+  Proof. hauto q:on inv:nat. Qed.
 
-  Lemma morphing_up n m (ρ0 ρ1 : fin n -> PTm m) :
+  Lemma morphing_up (ρ0 ρ1 : nat -> PTm) :
     (forall i, R (ρ0 i) (ρ1 i)) ->
     (forall i, R (up_PTm_PTm ρ0 i) (up_PTm_PTm ρ1 i)).
   Proof. hauto l:on ctrs:R use:morphing_ext, morphing_ren unfold:up_PTm_PTm. Qed.
 
-  Lemma morphing n m (a b : PTm n) (ρ0 ρ1 : fin n -> PTm m) :
+  Lemma morphing (a b : PTm) (ρ0 ρ1 : nat -> PTm) :
     (forall i, R (ρ0 i) (ρ1 i)) ->
     R a b -> R (subst_PTm ρ0 a) (subst_PTm ρ1 b).
   Proof.
-    move => + h. move : m ρ0 ρ1. elim : n a b / h => n.
-    move => a0 a1 ha iha m ρ0 ρ1 hρ /=.
+    move => + h. move : ρ0 ρ1. elim : a b / h.
+    move => a0 a1 ha iha ρ0 ρ1 hρ /=.
     eapply AppEta'; eauto. by asimpl.
     all : hauto lq:on ctrs:R use:morphing_up.
   Qed.
 
-  Lemma substing n m (a b : PTm n) (ρ : fin n -> PTm m) :
+  Lemma substing (a b : PTm) (ρ : nat -> PTm) :
     R a b -> R (subst_PTm ρ a) (subst_PTm ρ b).
   Proof. hauto l:on use:morphing, refl. Qed.
 
 End EPar.
 
-Inductive SNe {n} : PTm n -> Prop :=
+Inductive SNe : PTm -> Prop :=
 | N_Var i :
   SNe (VarPTm i)
 | N_App a b :
@@ -139,15 +137,13 @@ Inductive SNe {n} : PTm n -> Prop :=
 | N_Proj p a :
   SNe a ->
   SNe (PProj p a)
-| N_Bot :
-  SNe PBot
 | N_Ind P a b c :
   SN P ->
   SNe a ->
   SN b ->
   SN c ->
   SNe (PInd P a b c)
-with SN  {n} : PTm n -> Prop :=
+with SN  : PTm -> Prop :=
 | N_Pair a b :
   SN a ->
   SN b ->
@@ -175,7 +171,7 @@ with SN  {n} : PTm n -> Prop :=
 | N_Suc a :
   SN a ->
   SN (PSuc a)
-with TRedSN {n} : PTm n -> PTm n -> Prop :=
+with TRedSN : PTm -> PTm -> Prop :=
 | N_β a b :
   SN b ->
   TRedSN (PApp (PAbs a) b) (subst_PTm (scons b VarPTm) a)
@@ -210,38 +206,38 @@ with TRedSN {n} : PTm n -> PTm n -> Prop :=
   TRedSN a0 a1 ->
   TRedSN (PInd P a0 b c) (PInd P a1 b c).
 
-Derive Dependent Inversion tred_inv with (forall n (a b : PTm n), TRedSN a b) Sort Prop.
+Derive Inversion tred_inv with (forall (a b : PTm), TRedSN a b) Sort Prop.
 
-Inductive SNat {n} : PTm n -> Prop :=
+Inductive SNat : PTm -> Prop :=
 | S_Zero : SNat PZero
 | S_Neu a : SNe a -> SNat a
 | S_Suc a : SNat a -> SNat (PSuc a)
 | S_Red a b : TRedSN a b -> SNat b -> SNat a.
 
-Lemma PProj_imp n p a :
-  @ishf n a ->
+Lemma PProj_imp p a :
+  ishf a ->
   ~~ ispair a ->
   ~ SN (PProj p a).
 Proof.
   move => + + h. move E  : (PProj p a) h => u h.
   move : p a E.
-  elim : n u / h => //=.
+  elim : u / h => //=.
   hauto lq:on inv:SNe,PTm.
   hauto lq:on inv:TRedSN.
 Qed.
 
-Lemma PApp_imp n a b :
-  @ishf n a ->
+Lemma PApp_imp a b :
+  ishf a ->
   ~~ isabs a ->
   ~ SN (PApp a b).
 Proof.
   move => + + h. move E : (PApp a b) h => u h.
-  move : a b E. elim  : n u /h=>//=.
+  move : a b E. elim  : u /h=>//=.
   hauto lq:on inv:SNe,PTm.
   hauto lq:on inv:TRedSN.
 Qed.
 
-Lemma PInd_imp n P (a : PTm n) b c :
+Lemma PInd_imp P (a : PTm) b c :
   ishf a ->
   ~~ iszero a ->
   ~~ issuc a ->
@@ -249,35 +245,35 @@ Lemma PInd_imp n P (a : PTm n) b c :
 Proof.
   move => + + + h. move E : (PInd P a b c) h => u h.
   move : P a b c E.
-  elim : n u /h => //=.
+  elim : u /h => //=.
   hauto lq:on inv:SNe,PTm.
   hauto lq:on inv:TRedSN.
 Qed.
 
-Lemma PProjAbs_imp n p (a : PTm (S n)) :
+Lemma PProjAbs_imp p (a : PTm) :
   ~ SN (PProj p (PAbs a)).
 Proof.
   sfirstorder use:PProj_imp.
 Qed.
 
-Lemma PAppPair_imp n (a b0 b1 : PTm n ) :
+Lemma PAppPair_imp (a b0 b1 : PTm ) :
   ~ SN (PApp (PPair b0 b1) a).
 Proof.
   sfirstorder use:PApp_imp.
 Qed.
 
-Lemma PAppBind_imp n p (A : PTm n) B b :
+Lemma PAppBind_imp p (A : PTm) B b :
   ~ SN (PApp (PBind p A B) b).
 Proof.
   sfirstorder use:PApp_imp.
 Qed.
 
-Lemma PProjBind_imp n p p' (A : PTm n) B :
+Lemma PProjBind_imp p p' (A : PTm) B :
   ~ SN (PProj p (PBind p' A B)).
 Proof.
   move E :(PProj p (PBind p' A B)) => u hu.
   move : p p' A B E.
-  elim : n u /hu=>//=.
+  elim : u /hu=>//=.
   hauto lq:on inv:SNe.
   hauto lq:on inv:TRedSN.
 Qed.
@@ -288,7 +284,7 @@ Scheme sne_ind := Induction for SNe Sort Prop
 
 Combined Scheme sn_mutual from sne_ind, sn_ind, sred_ind.
 
-Fixpoint ne {n} (a : PTm n) :=
+Fixpoint ne (a : PTm) :=
   match a with
   | VarPTm i => true
   | PApp a b => ne a && nf b
@@ -297,13 +293,12 @@ Fixpoint ne {n} (a : PTm n) :=
   | PProj _ a => ne a
   | PUniv _ => false
   | PBind _ _ _ => false
-  | PBot => true
   | PInd P a b c => nf P && ne a && nf b && nf c
   | PNat => false
   | PSuc a => false
   | PZero => false
   end
-with nf {n} (a : PTm n) :=
+with nf (a : PTm) :=
   match a with
   | VarPTm i => true
   | PApp a b => ne a && nf b
@@ -312,69 +307,66 @@ with nf {n} (a : PTm n) :=
   | PProj _ a => ne a
   | PUniv _ => true
   | PBind _ A B => nf A && nf B
-  | PBot => true
   | PInd P a b c => nf P && ne a && nf b && nf c
   | PNat => true
   | PSuc a => nf a
   | PZero => true
 end.
 
-Lemma ne_nf n a : @ne n a -> nf a.
+Lemma ne_nf a : ne a -> nf a.
 Proof. elim : a => //=. Qed.
 
-Lemma ne_nf_ren n m (a : PTm n) (ξ : fin n -> fin m) :
+Lemma ne_nf_ren (a : PTm) (ξ : nat -> nat) :
   (ne a <-> ne (ren_PTm ξ a)) /\ (nf a <-> nf (ren_PTm ξ a)).
 Proof.
-  move : m ξ. elim : n / a => //=; solve [hauto b:on].
+  move : ξ. elim : a => //=; solve [hauto b:on].
 Qed.
 
-Inductive TRedSN' {n} (a : PTm n) : PTm n -> Prop :=
+Inductive TRedSN' (a : PTm) : PTm -> Prop :=
 | T_Refl :
   TRedSN' a a
 | T_Once b :
   TRedSN a b ->
   TRedSN' a b.
 
-Lemma SN_Proj n p (a : PTm n) :
+Lemma SN_Proj p (a : PTm) :
   SN (PProj p a) -> SN a.
 Proof.
   move E : (PProj p a) => u h.
   move : a E.
-  elim : n u / h => n //=; sauto.
+  elim : u / h => n //=; sauto.
 Qed.
 
-Lemma N_β' n a (b : PTm n) u :
+Lemma N_β' a (b : PTm) u :
   u = (subst_PTm (scons b VarPTm) a) ->
   SN b ->
   TRedSN (PApp (PAbs a) b) u.
 Proof. move => ->. apply N_β. Qed.
 
-Lemma N_IndSuc' n P a b c u :
+Lemma N_IndSuc' P a b c u :
   u = (subst_PTm (scons (PInd P a b c) (scons a VarPTm)) c) ->
   SN P ->
-  @SN n a ->
+  SN a ->
   SN b ->
   SN c ->
   TRedSN (PInd P (PSuc a) b c) u.
 Proof. move => ->. apply N_IndSuc. Qed.
 
-Lemma sn_renaming n :
-  (forall (a : PTm n) (s : SNe a), forall m (ξ : fin n -> fin m), SNe (ren_PTm ξ a)) /\
-  (forall (a : PTm n) (s : SN a), forall m (ξ : fin n -> fin m), SN (ren_PTm ξ a)) /\
-  (forall (a b : PTm n) (_ : TRedSN a b), forall m (ξ : fin n -> fin m), TRedSN (ren_PTm ξ a) (ren_PTm ξ b)).
+Lemma sn_renaming :
+  (forall (a : PTm) (s : SNe a), forall (ξ : nat -> nat), SNe (ren_PTm ξ a)) /\
+  (forall (a : PTm) (s : SN a), forall (ξ : nat -> nat), SN (ren_PTm ξ a)) /\
+  (forall (a b : PTm) (_ : TRedSN a b), forall (ξ : nat -> nat), TRedSN (ren_PTm ξ a) (ren_PTm ξ b)).
 Proof.
-  move : n. apply sn_mutual => n; try qauto ctrs:SN, SNe, TRedSN depth:1.
-  move => a b ha iha m ξ /=.
-  apply N_β'. by asimpl. eauto.
+  apply sn_mutual => n; try qauto ctrs:SN, SNe, TRedSN depth:1.
+  move => */=. apply N_β';eauto. by asimpl.
 
-  move => * /=.
-  apply N_IndSuc';eauto. by asimpl.
+  move => */=. apply N_IndSuc'; eauto. by asimpl.
 Qed.
 
-Lemma ne_nf_embed n (a : PTm n) :
+Lemma ne_nf_embed (a : PTm) :
   (ne a -> SNe a) /\ (nf a -> SN a).
 Proof.
-  elim : n  / a => //=; hauto qb:on ctrs:SNe, SN.
+  elim :  a => //=; hauto qb:on ctrs:SNe, SN.
 Qed.
 
 #[export]Hint Constructors SN SNe TRedSN : sn.
@@ -383,49 +375,53 @@ Ltac2 rec solve_anti_ren () :=
   let x := Fresh.in_goal (Option.get (Ident.of_string "x")) in
   intro $x;
   lazy_match! Constr.type (Control.hyp x) with
-  | fin _ -> _ _ => (ltac1:(case;qauto depth:2 db:sn))
+  | nat -> nat => (ltac1:(case;qauto depth:2 db:sn))
+  | nat -> PTm => (ltac1:(case;qauto depth:2 db:sn))
   | _ => solve_anti_ren ()
   end.
 
 Ltac solve_anti_ren := ltac2:(Control.enter solve_anti_ren).
 
-Lemma sn_antirenaming n :
-  (forall (a : PTm n) (s : SNe a), forall m (ξ : fin m -> fin n) b, a = ren_PTm ξ b -> SNe b) /\
-  (forall (a : PTm n) (s : SN a), forall m (ξ : fin m -> fin n) b, a = ren_PTm ξ b -> SN b) /\
-  (forall (a b : PTm n) (_ : TRedSN a b), forall m (ξ : fin m -> fin n) a0,
+Lemma sn_antirenaming :
+  (forall (a : PTm) (s : SNe a), forall (ξ : nat -> nat) b, a = ren_PTm ξ b -> SNe b) /\
+  (forall (a : PTm) (s : SN a), forall (ξ : nat -> nat) b, a = ren_PTm ξ b -> SN b) /\
+  (forall (a b : PTm) (_ : TRedSN a b), forall (ξ : nat -> nat) a0,
       a = ren_PTm ξ a0 -> exists b0, TRedSN a0 b0 /\ b = ren_PTm ξ b0).
 Proof.
-  move : n. apply sn_mutual => n; try solve_anti_ren.
+  apply sn_mutual; try solve_anti_ren.
+  move => *. subst. spec_refl. hauto lq:on ctrs:TRedSN, SN.
 
-  move => a b ha iha m ξ []//= u u0 [+ ?]. subst.
+  move => a b ha iha ξ []//= u u0 [+ ?]. subst.
   case : u => //= => u [*]. subst.
   spec_refl. eexists. split. apply N_β=>//. by asimpl.
 
-  move => a b hb ihb m ξ[]//= p p0 [? +]. subst.
+  move => a b hb ihb ξ[]//= p p0 [? +]. subst.
   case : p0 => //= p p0 [*]. subst.
   spec_refl. by eauto with sn.
 
-  move => a b ha iha m ξ[]//= u u0 [? ]. subst.
+  move => a b ha iha ξ[]//= u u0 [? ]. subst.
   case : u0 => //=. move => p p0 [*]. subst.
   spec_refl. by eauto with sn.
 
-  move => P b c ha iha hb ihb hc ihc m ξ []//= P0 a0 b0 c0 [?]. subst.
+  move => P b c ha iha hb ihb hc ihc ξ []//= P0 a0 b0 c0 [?]. subst.
   case : a0 => //= _ *. subst.
   spec_refl. by eauto with sn.
 
-  move => P a b c hP ihP ha iha hb ihb hc ihc m ξ []//= P0 a0 b0 c0 [?]. subst.
+  move => P a b c hP ihP ha iha hb ihb hc ihc ξ []//= P0 a0 b0 c0 [?]. subst.
   case : a0 => //= a0 [*]. subst.
   spec_refl. eexists; repeat split; eauto with sn.
-  by asimpl. Qed.
+  by asimpl.
+Qed.
 
-Lemma sn_unmorphing n :
-  (forall (a : PTm n) (s : SNe a), forall m (ρ : fin m -> PTm n) b, a = subst_PTm ρ b -> SNe b) /\
-  (forall (a : PTm n) (s : SN a), forall m (ρ : fin m -> PTm n) b, a = subst_PTm ρ b -> SN b) /\
-  (forall (a b : PTm n) (_ : TRedSN a b), forall m (ρ : fin m -> PTm n) a0,
+Lemma sn_unmorphing :
+  (forall (a : PTm) (s : SNe a), forall (ρ : nat -> PTm) b, a = subst_PTm ρ b -> SNe b) /\
+  (forall (a : PTm) (s : SN a), forall (ρ : nat -> PTm) b, a = subst_PTm ρ b -> SN b) /\
+  (forall (a b : PTm) (_ : TRedSN a b), forall (ρ : nat -> PTm) a0,
       a = subst_PTm ρ a0 -> (exists b0, b = subst_PTm ρ b0 /\ TRedSN a0 b0) \/ SNe a0).
 Proof.
-  move : n. apply sn_mutual => n; try solve_anti_ren.
-  - move => a b ha iha  m ξ b0.
+  apply sn_mutual; try solve_anti_ren.
+  - hauto q:on db:sn.
+  - move => a b ha iha  ξ b0.
     case : b0 => //=.
     + hauto lq:on rew:off db:sn.
     + move => p p0 [+ ?]. subst.
@@ -436,7 +432,7 @@ Proof.
       spec_refl.
       eexists. split; last by eauto using N_β.
       by asimpl.
-  - move => a0 a1 b hb ihb ha iha m ρ []//=.
+  - move => a0 a1 b hb ihb ha iha ρ []//=.
     + hauto lq:on rew:off db:sn.
     + move => t0  t1 [*]. subst.
       spec_refl.
@@ -447,18 +443,18 @@ Proof.
       * move => h.
         right.
         apply N_App => //.
-  - move => a b hb ihb m ρ []//=.
+  - move => a b hb ihb ρ []//=.
     + hauto l:on ctrs:TRedSN.
     + move => p p0 [?]. subst.
       case : p0 => //=.
       * hauto lq:on rew:off db:sn.
       * move => p p0 [*]. subst.
         hauto lq:on db:sn.
-  - move => a b ha iha m ρ []//=; first by hauto l:on db:sn.
+  - move => a b ha iha ρ []//=; first by hauto l:on db:sn.
     case => //=. move => []//=.
     + hauto lq:on db:sn.
     + hauto lq:on db:sn.
-  - move => p a b ha iha m ρ []//=; first by hauto l:on db:sn.
+  - move => p a b ha iha ρ []//=; first by hauto l:on db:sn.
     move => t0 t1 [*]. subst.
     spec_refl.
     case : iha.
@@ -466,12 +462,12 @@ Proof.
       left. eexists. split; last by eauto with sn.
       reflexivity.
     + hauto lq:on db:sn.
-  - move => P b c hP ihP hb ihb hc ihc m ρ []//=.
+  - move => P b c hP ihP hb ihb hc ihc ρ []//=.
     + hauto lq:on db:sn.
     + move => p []//=.
       * hauto lq:on db:sn.
       * hauto q:on db:sn.
-  - move => P a b c hP ihP ha iha hb ihb hc ihc m ρ []//=.
+  - move => P a b c hP ihP ha iha hb ihb hc ihc ρ []//=.
     + hauto lq:on db:sn.
     + move => P0 a0 b0 c0 [?]. subst.
       case : a0 => //=.
@@ -480,7 +476,7 @@ Proof.
         spec_refl.
         left. eexists. split; last by eauto with sn.
         by asimpl.
-  - move => P a0 a1 b c hP ihP hb ihb hc ihc ha iha m ρ[]//=.
+  - move => P a0 a1 b c hP ihP hb ihb hc ihc ha iha ρ[]//=.
     + hauto lq:on db:sn.
     + move => P1 a2 b2 c2 [*]. subst.
       spec_refl.
@@ -491,42 +487,41 @@ Proof.
       * hauto lq:on db:sn.
 Qed.
 
-Lemma SN_AppInv : forall n (a b : PTm n), SN (PApp a b) -> SN a /\ SN b.
+Lemma SN_AppInv : forall (a b : PTm), SN (PApp a b) -> SN a /\ SN b.
 Proof.
-  move => n a b. move E : (PApp a b) => u hu. move : a b E.
-  elim : n u /hu=>//=.
+  move => a b. move E : (PApp a b) => u hu. move : a b E.
+  elim : u /hu=>//=.
   hauto lq:on rew:off inv:SNe db:sn.
-  move => n a b ha hb ihb a0 b0 ?. subst.
+  move => a b ha hb ihb a0 b0 ?. subst.
   inversion ha; subst.
   move {ihb}.
   hecrush use:sn_unmorphing.
   hauto lq:on db:sn.
 Qed.
 
-Lemma SN_ProjInv : forall n p (a : PTm n), SN (PProj p a) -> SN a.
+Lemma SN_ProjInv : forall p (a : PTm), SN (PProj p a) -> SN a.
 Proof.
-  move => n p a. move E : (PProj p a) => u hu.
+  move => p a. move E : (PProj p a) => u hu.
   move : p a E.
-  elim : n u / hu => //=.
+  elim : u / hu => //=.
   hauto lq:on rew:off inv:SNe db:sn.
   hauto lq:on rew:off inv:TRedSN db:sn.
 Qed.
 
-Lemma SN_IndInv : forall n P (a : PTm n) b c, SN (PInd P a b c) -> SN P /\ SN a /\ SN b /\ SN c.
+Lemma SN_IndInv : forall P (a : PTm) b c, SN (PInd P a b c) -> SN P /\ SN a /\ SN b /\ SN c.
 Proof.
-  move => n P a b c. move E : (PInd P a b c) => u hu. move : P a b c E.
-  elim  : n u / hu => //=.
+  move => P a b c. move E : (PInd P a b c) => u hu. move : P a b c E.
+  elim  : u / hu => //=.
   hauto lq:on rew:off inv:SNe db:sn.
   hauto lq:on rew:off inv:TRedSN db:sn.
 Qed.
 
-Lemma epar_sn_preservation n :
-  (forall (a : PTm n) (s : SNe a), forall b, EPar.R a b -> SNe b) /\
-  (forall (a : PTm n) (s : SN a), forall b, EPar.R a b -> SN b) /\
-  (forall (a b : PTm n) (_ : TRedSN a b), forall c, EPar.R a c -> exists d, TRedSN' c d /\ EPar.R b d).
+Lemma epar_sn_preservation :
+  (forall (a : PTm) (s : SNe a), forall b, EPar.R a b -> SNe b) /\
+  (forall (a : PTm) (s : SN a), forall b, EPar.R a b -> SN b) /\
+  (forall (a b : PTm) (_ : TRedSN a b), forall c, EPar.R a c -> exists d, TRedSN' c d /\ EPar.R b d).
 Proof.
-  move : n. apply sn_mutual => n.
-  - sauto lq:on.
+  apply sn_mutual.
   - sauto lq:on.
   - sauto lq:on.
   - sauto lq:on.
@@ -562,7 +557,7 @@ Proof.
       exists (subst_PTm (scons b1 VarPTm) a2).
       split.
       sauto lq:on.
-      hauto lq:on use:EPar.morphing, EPar.refl inv:option.
+      hauto lq:on use:EPar.morphing, EPar.refl inv:nat.
   - sauto.
   - move => a b hb ihb c.
     elim /EPar.inv => //= _.
@@ -590,12 +585,12 @@ Proof.
     elim /EPar.inv : ha0 => //=_.
     move => a0 a2 ha0 [*]. subst.
     eexists. split. apply T_Once. apply N_IndSuc; eauto.
-    hauto q:on ctrs:EPar.R use:EPar.morphing, EPar.refl inv:option.
+    hauto q:on ctrs:EPar.R use:EPar.morphing, EPar.refl inv:nat.
   - sauto q:on.
 Qed.
 
 Module RRed.
-  Inductive R {n} : PTm n -> PTm n ->  Prop :=
+  Inductive R : PTm -> PTm ->  Prop :=
   (****************** Beta ***********************)
   | AppAbs a b :
     R (PApp (PAbs a) b)  (subst_PTm (scons b VarPTm) a)
@@ -649,27 +644,27 @@ Module RRed.
     R a0 a1 ->
     R (PSuc a0) (PSuc a1).
 
-  Derive Dependent Inversion inv with (forall n (a b : PTm n), R a b) Sort Prop.
+  Derive Inversion inv with (forall (a b : PTm), R a b) Sort Prop.
 
-  Lemma AppAbs' n a (b : PTm n) u :
+  Lemma AppAbs' a (b : PTm) u :
     u = (subst_PTm (scons b VarPTm) a) ->
     R (PApp (PAbs a) b)  u.
   Proof.
     move => ->. by apply AppAbs. Qed.
 
-  Lemma IndSuc' n P a b c u :
+  Lemma IndSuc' P a b c u :
     u = (subst_PTm (scons (PInd P a b c) (scons a VarPTm)) c) ->
-    R (@PInd n P (PSuc a) b c) u.
+    R (PInd P (PSuc a) b c) u.
   Proof. move => ->. apply IndSuc. Qed.
 
-  Lemma renaming n m (a b : PTm n) (ξ : fin n -> fin m) :
+  Lemma renaming (a b : PTm) (ξ : nat -> nat) :
     R a b -> R (ren_PTm ξ a) (ren_PTm ξ b).
   Proof.
-    move => h. move : m ξ.
-    elim : n a b /h.
+    move => h. move : ξ.
+    elim : a b /h.
 
     all : try qauto ctrs:R.
-    move => n a b m ξ /=.
+    move => a b ξ /=.
     apply AppAbs'. by asimpl.
     move => */=; apply IndSuc'; eauto. by asimpl.
   Qed.
@@ -678,56 +673,56 @@ Module RRed.
     let x := Fresh.in_goal (Option.get (Ident.of_string "x")) in
     intro $x;
     lazy_match! Constr.type (Control.hyp x) with
-    | fin _ -> _ _ => (ltac1:(case;hauto q:on depth:2 ctrs:RRed.R))
+    | nat -> nat => (ltac1:(case;hauto q:on depth:2 ctrs:RRed.R))
+    | nat -> PTm => (ltac1:(case;hauto q:on depth:2 ctrs:RRed.R))
     | _ => solve_anti_ren ()
     end.
 
   Ltac solve_anti_ren := ltac2:(Control.enter solve_anti_ren).
 
-  Lemma antirenaming n m (a : PTm n) (b : PTm m) (ξ : fin n -> fin m) :
+  Lemma antirenaming (a : PTm) (b : PTm) (ξ : nat -> nat) :
     R (ren_PTm ξ a) b -> exists b0, R a b0 /\ ren_PTm ξ b0 = b.
   Proof.
     move E : (ren_PTm ξ a) => u h.
-    move : n ξ a E. elim : m u b/h; try solve_anti_ren.
-    - move => n a b m ξ []//=. move => []//= t t0 [*]. subst.
+    move : ξ a E. elim : u b/h; try solve_anti_ren.
+    - move => a b ξ []//=. move => []//= t t0 [*]. subst.
       eexists. split. apply AppAbs. by asimpl.
-    - move => n p a b m ξ []//=.
+    - move => p a b ξ []//=.
       move => p0 []//=. hauto q:on ctrs:R.
-    - move => n p b c m ξ []//= P a0 b0 c0 [*]. subst.
+    - move => p b c ξ []//= P a0 b0 c0 [*]. subst.
       destruct a0 => //=.
       hauto lq:on ctrs:R.
-    - move => n P a b c m ξ []//=.
+    - move => P a b c ξ []//=.
       move => p p0 p1 p2 [?].  subst.
       case : p0 => //=.
       move => p0 [?] *. subst. eexists. split; eauto using IndSuc.
       by asimpl.
   Qed.
 
-  Lemma nf_imp n (a b : PTm n) :
+  Lemma nf_imp (a b : PTm) :
     nf a ->
     R a b -> False.
   Proof. move/[swap]. induction 1; hauto qb:on inv:PTm. Qed.
 
-  Lemma FromRedSN n (a b : PTm n) :
+  Lemma FromRedSN (a b : PTm) :
     TRedSN a b ->
     RRed.R a b.
   Proof. induction 1; hauto lq:on ctrs:RRed.R. Qed.
 
-  Lemma substing n m (a b : PTm n) (ρ : fin n -> PTm m) :
+  Lemma substing (a b : PTm) (ρ : nat -> PTm) :
     R a b -> R (subst_PTm ρ a) (subst_PTm ρ b).
   Proof.
-    move => h. move : m ρ. elim : n a b / h => n.
+    move => h. move :  ρ. elim : a b / h => n.
 
     all : try hauto lq:on ctrs:R.
-    move => a b m ρ /=.
-    eapply AppAbs'; eauto; cycle 1. by asimpl.
+    move => */=. eapply AppAbs'; eauto; cycle 1. by asimpl.
     move => */=; apply : IndSuc'; eauto. by asimpl.
   Qed.
 
 End RRed.
 
 Module RPar.
-  Inductive R {n} : PTm n -> PTm n ->  Prop :=
+  Inductive R : PTm -> PTm ->  Prop :=
   (****************** Beta ***********************)
   | AppAbs a0 a1 b0 b1 :
     R a0 a1 ->
@@ -774,8 +769,6 @@ Module RPar.
     R A0 A1 ->
     R B0 B1 ->
     R (PBind p A0 B0) (PBind p A1 B1)
-  | BotCong :
-    R PBot PBot
   | NatCong :
     R PNat PNat
   | IndCong P0 P1 a0 a1 b0 b1 c0 c1 :
@@ -792,28 +785,28 @@ Module RPar.
     (* ------------ *)
     R (PSuc a0) (PSuc a1).
 
-  Lemma refl n (a : PTm n) : R a a.
+  Lemma refl (a : PTm) : R a a.
   Proof.
-    elim : n / a; hauto lq:on ctrs:R.
+    elim : a; hauto lq:on ctrs:R.
   Qed.
 
-  Derive Dependent Inversion inv with (forall n (a b : PTm n), R a b) Sort Prop.
+  Derive Dependent Inversion inv with (forall (a b : PTm), R a b) Sort Prop.
 
-  Lemma AppAbs' n a0 a1 (b0 b1 : PTm n) u :
+  Lemma AppAbs' a0 a1 (b0 b1 : PTm) u :
     u = (subst_PTm (scons b1 VarPTm) a1) ->
     R a0 a1 ->
     R b0 b1 ->
     R (PApp (PAbs a0) b0)  u.
   Proof. move => ->. apply AppAbs. Qed.
 
-  Lemma ProjPair' n p u (a0 a1 b0 b1 : PTm n) :
+  Lemma ProjPair' p u (a0 a1 b0 b1 : PTm) :
     u = (if p is PL then a1 else b1) ->
     R a0 a1 ->
     R b0 b1 ->
     R (PProj p (PPair a0 b0)) u.
   Proof. move => ->. apply ProjPair. Qed.
 
-  Lemma IndSuc' n P0 P1 (a0 a1 : PTm n) b0 b1 c0 c1 u :
+  Lemma IndSuc' P0 P1 (a0 a1 : PTm) b0 b1 c0 c1 u :
     u = (subst_PTm (scons (PInd P1 a1 b1 c1) (scons a1 VarPTm)) c1) ->
     R P0 P1 ->
     R a0 a1 ->
@@ -823,43 +816,43 @@ Module RPar.
     R (PInd P0 (PSuc a0) b0 c0) u.
   Proof. move => ->. apply IndSuc. Qed.
 
-  Lemma renaming n m (a b : PTm n) (ξ : fin n -> fin m) :
+  Lemma renaming (a b : PTm) (ξ : nat -> nat) :
     R a b -> R (ren_PTm ξ a) (ren_PTm ξ b).
   Proof.
-    move => h. move : m ξ.
-    elim : n a b /h.
+    move => h. move : ξ.
+    elim : a b /h.
 
     all : try qauto ctrs:R use:ProjPair'.
 
-    move => n a0 a1 b0 b1 ha iha hb ihb m ξ /=.
+    move => a0 a1 b0 b1 ha iha hb ihb ξ /=.
     eapply AppAbs'; eauto. by asimpl.
 
     move => * /=. apply : IndSuc'; eauto. by asimpl.
   Qed.
 
-  Lemma morphing_ren n m p (ρ0 ρ1 : fin n -> PTm m) (ξ : fin m -> fin p) :
+  Lemma morphing_ren (ρ0 ρ1 : nat -> PTm) (ξ : nat -> nat) :
     (forall i, R (ρ0 i) (ρ1 i)) ->
     (forall i, R ((funcomp (ren_PTm ξ) ρ0) i) ((funcomp (ren_PTm ξ) ρ1) i)).
   Proof. eauto using renaming. Qed.
 
-  Lemma morphing_ext n m (ρ0 ρ1 : fin n -> PTm m) a b  :
+  Lemma morphing_ext (ρ0 ρ1 : nat -> PTm) a b  :
     R a b ->
     (forall i, R (ρ0 i) (ρ1 i)) ->
     (forall i, R ((scons a ρ0) i) ((scons b ρ1) i)).
-  Proof. hauto q:on inv:option. Qed.
+  Proof. hauto q:on inv:nat. Qed.
 
-  Lemma morphing_up n m (ρ0 ρ1 : fin n -> PTm m) :
+  Lemma morphing_up (ρ0 ρ1 : nat -> PTm) :
     (forall i, R (ρ0 i) (ρ1 i)) ->
     (forall i, R (up_PTm_PTm ρ0 i) (up_PTm_PTm ρ1 i)).
   Proof. hauto l:on ctrs:R use:morphing_ext, morphing_ren unfold:up_PTm_PTm. Qed.
 
-  Lemma morphing n m (a b : PTm n) (ρ0 ρ1 : fin n -> PTm m) :
+  Lemma morphing (a b : PTm) (ρ0 ρ1 : nat -> PTm) :
     (forall i, R (ρ0 i) (ρ1 i)) ->
     R a b -> R (subst_PTm ρ0 a) (subst_PTm ρ1 b).
   Proof.
-    move => + h. move : m ρ0 ρ1. elim : n a b / h => n.
+    move => + h. move : ρ0 ρ1. elim : a b / h.
     all : try hauto lq:on ctrs:R use:morphing_up, ProjPair'.
-    move => a0 a1 b0 b1 ha iha hb ihb m ρ0 ρ1 hρ /=.
+    move => a0 a1 b0 b1 ha iha hb ihb ρ0 ρ1 hρ /=.
     eapply AppAbs'; eauto; cycle 1. sfirstorder use:morphing_up. by asimpl.
     move => */=; eapply IndSuc'; eauto; cycle 1.
     sfirstorder use:morphing_up.
@@ -867,29 +860,29 @@ Module RPar.
     by asimpl.
   Qed.
 
-  Lemma substing n m (a : PTm n) b (ρ : fin n -> PTm m) :
+  Lemma substing (a : PTm) b (ρ : nat -> PTm) :
     R a b ->
     R (subst_PTm ρ a) (subst_PTm ρ b).
   Proof.
     hauto l:on use:morphing, refl.
   Qed.
 
-  Lemma cong n (a0 a1 : PTm (S n)) b0 b1  :
+  Lemma cong (a0 a1 : PTm) b0 b1  :
     R a0 a1 ->
     R b0 b1 ->
     R (subst_PTm (scons b0 VarPTm) a0) (subst_PTm (scons b1 VarPTm) a1).
   Proof.
     move => h0 h1. apply morphing=>//.
-    hauto q:on inv:option ctrs:R.
+    hauto q:on inv:nat ctrs:R.
   Qed.
 
-  Lemma FromRRed n (a b : PTm n) :
+  Lemma FromRRed (a b : PTm) :
     RRed.R a b -> RPar.R a b.
   Proof.
     induction 1; qauto l:on use:RPar.refl ctrs:RPar.R.
   Qed.
 
-  Function tstar {n} (a : PTm n) :=
+  Function tstar (a : PTm) :=
     match a with
     | VarPTm i => a
     | PAbs a => PAbs (tstar a)
@@ -900,7 +893,6 @@ Module RPar.
     | PProj p a => PProj p (tstar a)
     | PUniv i => PUniv i
     | PBind p A B => PBind p (tstar A) (tstar B)
-    | PBot => PBot
     | PNat => PNat
     | PZero => PZero
     | PSuc a => PSuc (tstar a)
@@ -910,11 +902,11 @@ Module RPar.
     | PInd P a b c => PInd (tstar P) (tstar a) (tstar b) (tstar c)
     end.
 
-  Lemma triangle n (a b : PTm n) :
+  Lemma triangle (a b : PTm) :
     RPar.R a b -> RPar.R b (tstar a).
   Proof.
     move : b.
-    apply tstar_ind => {}n{}a.
+    apply tstar_ind => {}a.
     - hauto lq:on ctrs:R inv:R.
     - hauto lq:on ctrs:R inv:R.
     - hauto lq:on rew:off inv:R use:cong ctrs:R.
@@ -942,33 +934,31 @@ Module RPar.
     - hauto lq:on ctrs:R inv:R.
     - hauto lq:on ctrs:R inv:R.
     - hauto lq:on ctrs:R inv:R.
-    - move => P b c ?. subst.
-      move => h0. inversion 1; subst. hauto lq:on ctrs:R. qauto l:on inv:R ctrs:R.
     - move => P a0 b c ? hP ihP ha iha hb ihb u. subst.
       elim /inv => //= _.
       + move => P0 P1 a1 a2 b0 b1 c0 c1 hP' ha' hb' hc' [*]. subst.
-        apply morphing. hauto lq:on ctrs:R inv:option.
+        apply morphing. hauto lq:on ctrs:R inv:nat.
         eauto.
       + sauto q:on ctrs:R.
     - sauto lq:on.
   Qed.
 
-  Lemma diamond n (a b c : PTm n) :
+  Lemma diamond (a b c : PTm) :
     R a b -> R a c -> exists d, R b d /\ R c d.
   Proof. eauto using triangle. Qed.
 End RPar.
 
-Lemma red_sn_preservation n :
-  (forall (a : PTm n) (s : SNe a), forall b, RPar.R a b -> SNe b) /\
-  (forall (a : PTm n) (s : SN a), forall b, RPar.R a b -> SN b) /\
-  (forall (a b : PTm n) (_ : TRedSN a b), forall c, RPar.R a c -> exists d, TRedSN' c d /\ RPar.R b d).
+Lemma red_sn_preservation :
+  (forall (a : PTm) (s : SNe a), forall b, RPar.R a b -> SNe b) /\
+  (forall (a : PTm) (s : SN a), forall b, RPar.R a b -> SN b) /\
+  (forall (a b : PTm) (_ : TRedSN a b), forall c, RPar.R a c -> exists d, TRedSN' c d /\ RPar.R b d).
 Proof.
-  move : n. apply sn_mutual => n.
+  apply sn_mutual.
   - hauto l:on inv:RPar.R.
   - qauto l:on inv:RPar.R,SNe,SN ctrs:SNe.
   - hauto lq:on inv:RPar.R, SNe ctrs:SNe.
   - hauto lq:on inv:RPar.R, SNe ctrs:SNe.
-  - qauto l:on inv:RPar.R, SN,SNe ctrs:SNe.
+  (* - qauto l:on inv:RPar.R, SN,SNe ctrs:SNe. *)
   - qauto l:on ctrs:SN inv:RPar.R.
   - hauto lq:on ctrs:SN inv:RPar.R.
   - hauto lq:on ctrs:SN.
@@ -1002,13 +992,13 @@ Proof.
     elim /RPar.inv => //=_.
     + move => P0 P1 a0 a1 b0 b1 c0 c1 hP' ha' hb' hc' [*]. subst.
       eexists. split; first by apply T_Refl.
-      apply RPar.morphing=>//. hauto lq:on ctrs:RPar.R inv:option.
+      apply RPar.morphing=>//. hauto lq:on ctrs:RPar.R inv:nat.
     + move => P0 P1 a0 a1 b0 b1 c0 c1 hP' ha' hb' hc' [*]. subst.
       elim /RPar.inv : ha' => //=_.
       move => a0 a2 ha' [*]. subst.
       eexists. split. apply T_Once.
       apply N_IndSuc; eauto.
-      hauto q:on use:RPar.morphing ctrs:RPar.R inv:option.
+      hauto q:on use:RPar.morphing ctrs:RPar.R inv:nat.
   - sauto q:on.
 Qed.
 
@@ -1021,34 +1011,34 @@ Module RReds.
   #[local]Ltac solve_s :=
     repeat (induction 1; last by solve_s_rec); apply rtc_refl.
 
-  Lemma AbsCong n (a b : PTm (S n)) :
+  Lemma AbsCong (a b : PTm) :
     rtc RRed.R a b ->
     rtc RRed.R (PAbs a) (PAbs b).
   Proof. solve_s. Qed.
 
-  Lemma AppCong n (a0 a1 b0 b1 : PTm n) :
+  Lemma AppCong (a0 a1 b0 b1 : PTm) :
     rtc RRed.R a0 a1 ->
     rtc RRed.R b0 b1 ->
     rtc RRed.R (PApp a0 b0) (PApp a1 b1).
   Proof. solve_s. Qed.
 
-  Lemma PairCong n (a0 a1 b0 b1 : PTm n) :
+  Lemma PairCong (a0 a1 b0 b1 : PTm) :
     rtc RRed.R a0 a1 ->
     rtc RRed.R b0 b1 ->
     rtc RRed.R (PPair a0 b0) (PPair a1 b1).
   Proof. solve_s. Qed.
 
-  Lemma ProjCong n p (a0 a1  : PTm n) :
+  Lemma ProjCong p (a0 a1  : PTm) :
     rtc RRed.R a0 a1 ->
     rtc RRed.R (PProj p a0) (PProj p a1).
   Proof. solve_s. Qed.
 
-  Lemma SucCong n (a0 a1 : PTm n) :
+  Lemma SucCong (a0 a1 : PTm) :
     rtc RRed.R a0 a1 ->
     rtc RRed.R (PSuc a0) (PSuc a1).
   Proof. solve_s. Qed.
 
-  Lemma IndCong n P0 P1 (a0 a1 : PTm n) b0 b1 c0 c1 :
+  Lemma IndCong P0 P1 (a0 a1 : PTm) b0 b1 c0 c1 :
     rtc RRed.R P0 P1 ->
     rtc RRed.R a0 a1 ->
     rtc RRed.R b0 b1 ->
@@ -1056,27 +1046,27 @@ Module RReds.
     rtc RRed.R (PInd P0 a0 b0 c0) (PInd P1 a1 b1 c1).
   Proof. solve_s. Qed.
 
-  Lemma BindCong n p (A0 A1 : PTm n) B0 B1 :
+  Lemma BindCong p (A0 A1 : PTm) B0 B1 :
     rtc RRed.R A0 A1 ->
     rtc RRed.R B0 B1 ->
     rtc RRed.R (PBind p A0 B0) (PBind p A1 B1).
   Proof. solve_s. Qed.
 
-  Lemma renaming n m (a b : PTm n) (ξ : fin n -> fin m) :
+  Lemma renaming (a b : PTm) (ξ : nat -> nat) :
     rtc RRed.R a b -> rtc RRed.R (ren_PTm ξ a) (ren_PTm ξ b).
   Proof.
-    move => h. move : m ξ. elim : a b /h; hauto lq:on ctrs:rtc use:RRed.renaming.
+    move => h. move : ξ. elim : a b /h; hauto lq:on ctrs:rtc use:RRed.renaming.
   Qed.
 
-  Lemma FromRPar n (a b : PTm n) (h : RPar.R a b) :
+  Lemma FromRPar (a b : PTm) (h : RPar.R a b) :
     rtc RRed.R a b.
   Proof.
-    elim : n a b /h; eauto using AbsCong, AppCong, PairCong, ProjCong, rtc_refl, BindCong, IndCong, SucCong.
-    move => n a0 a1 b0 b1 ha iha hb ihb.
+    elim : a b /h; eauto using AbsCong, AppCong, PairCong, ProjCong, rtc_refl, BindCong, IndCong, SucCong.
+    move => a0 a1 b0 b1 ha iha hb ihb.
     apply : rtc_r; last by apply RRed.AppAbs.
     by eauto using AppCong, AbsCong.
 
-    move => n p a0 a1 b0 b1 ha iha hb ihb.
+    move => p a0 a1 b0 b1 ha iha hb ihb.
     apply : rtc_r; last by apply RRed.ProjPair.
     by eauto using PairCong, ProjCong.
 
@@ -1087,7 +1077,7 @@ Module RReds.
     by eauto using SucCong, IndCong.
   Qed.
 
-  Lemma RParIff n (a b : PTm n) :
+  Lemma RParIff (a b : PTm) :
     rtc RRed.R a b <-> rtc RPar.R a b.
   Proof.
     split.
@@ -1095,11 +1085,11 @@ Module RReds.
     induction 1; hauto l:on ctrs:rtc use:FromRPar, @relations.rtc_transitive.
   Qed.
 
-  Lemma nf_refl n (a b : PTm n) :
+  Lemma nf_refl (a b : PTm) :
     rtc RRed.R a b -> nf a -> a = b.
   Proof. induction 1; sfirstorder use:RRed.nf_imp. Qed.
 
-  Lemma FromRedSNs n (a b : PTm n) :
+  Lemma FromRedSNs (a b : PTm) :
     rtc TRedSN a b ->
     rtc RRed.R a b.
   Proof. induction 1; hauto lq:on ctrs:rtc use:RRed.FromRedSN. Qed.
@@ -1108,7 +1098,7 @@ End RReds.
 
 
 Module NeEPar.
-  Inductive R_nonelim {n} : PTm n -> PTm n ->  Prop :=
+  Inductive R_nonelim : PTm -> PTm ->  Prop :=
   (****************** Eta ***********************)
   | AppEta a0 a1 :
     ~~ ishf a0 ->
@@ -1141,8 +1131,6 @@ Module NeEPar.
     R_nonelim A0 A1 ->
     R_nonelim B0 B1 ->
     R_nonelim (PBind p A0 B0) (PBind p A1 B1)
-  | BotCong :
-    R_nonelim PBot PBot
   | NatCong :
     R_nonelim PNat PNat
   | IndCong P0 P1 a0 a1 b0 b1 c0 c1 :
@@ -1158,7 +1146,7 @@ Module NeEPar.
     R_nonelim a0 a1 ->
     (* ------------ *)
     R_nonelim (PSuc a0) (PSuc a1)
-  with R_elim {n} : PTm n -> PTm n -> Prop :=
+  with R_elim : PTm -> PTm -> Prop :=
   | NAbsCong a0 a1 :
     R_nonelim a0 a1 ->
     R_elim (PAbs a0) (PAbs a1)
@@ -1181,8 +1169,6 @@ Module NeEPar.
     R_nonelim A0 A1 ->
     R_nonelim B0 B1 ->
     R_elim (PBind p A0 B0) (PBind p A1 B1)
-  | NBotCong :
-    R_elim PBot PBot
   | NNatCong :
     R_elim PNat PNat
   | NIndCong P0 P1 a0 a1 b0 b1 c0 c1 :
@@ -1204,11 +1190,11 @@ Module NeEPar.
 
   Combined Scheme epar_mutual from epar_elim_ind, epar_nonelim_ind.
 
-  Lemma R_elim_nf n :
-    (forall (a b : PTm n), R_elim a b -> nf b -> nf a) /\
-      (forall (a b : PTm n), R_nonelim a b -> nf b -> nf a).
+  Lemma R_elim_nf :
+    (forall (a b : PTm), R_elim a b -> nf b -> nf a) /\
+      (forall (a b : PTm), R_nonelim a b -> nf b -> nf a).
   Proof.
-    move : n. apply epar_mutual => n //=.
+    apply epar_mutual => //=.
     - move => a0 a1 b0 b1 h ih h' ih' /andP [h0 h1].
       have hb0 : nf b0 by eauto.
       suff : ne a0 by qauto b:on.
@@ -1237,22 +1223,22 @@ Module NeEPar.
     - hauto lqb:on inv:R_elim.
   Qed.
 
-  Lemma R_nonelim_nothf n (a b : PTm n) :
+  Lemma R_nonelim_nothf (a b : PTm) :
     R_nonelim a b ->
     ~~ ishf a ->
     R_elim a b.
   Proof.
-    move => h. elim : n a b /h=>//=; hauto lq:on ctrs:R_elim.
+    move => h. elim : a b /h=>//=; hauto lq:on ctrs:R_elim.
   Qed.
 
-  Lemma R_elim_nonelim n (a b : PTm n) :
+  Lemma R_elim_nonelim (a b : PTm) :
     R_elim a b ->
     R_nonelim a b.
-    move => h. elim : n a b /h=>//=; hauto lq:on ctrs:R_nonelim.
+    move => h. elim : a b /h=>//=; hauto lq:on ctrs:R_nonelim.
   Qed.
 
-  Lemma ToEPar : forall n, (forall (a b : PTm n), R_elim a b -> EPar.R a b) /\
-                 (forall (a b : PTm n), R_nonelim a b -> EPar.R a b).
+  Lemma ToEPar : (forall (a b : PTm), R_elim a b -> EPar.R a b) /\
+                 (forall (a b : PTm), R_nonelim a b -> EPar.R a b).
   Proof.
     apply epar_mutual; qauto l:on ctrs:EPar.R.
   Qed.
@@ -1260,51 +1246,45 @@ Module NeEPar.
 End NeEPar.
 
 Module Type NoForbid.
-  Parameter P : forall n, PTm n -> Prop.
-  Arguments P {n}.
+  Parameter P : PTm -> Prop.
 
-  Axiom P_EPar : forall n (a b : PTm n), EPar.R a b -> P a -> P b.
-  Axiom P_RRed : forall n (a b : PTm n), RRed.R a b -> P a -> P b.
-  (* Axiom P_AppPair : forall n (a b c : PTm n), ~ P (PApp (PPair a b) c). *)
-  (* Axiom P_ProjAbs : forall n p (a : PTm (S n)), ~ P (PProj p (PAbs a)). *)
-  (* Axiom P_ProjBind : forall n p p' (A : PTm n) B, ~ P (PProj p (PBind p' A B)). *)
-  (* Axiom P_AppBind : forall n p (A : PTm n) B b, ~ P (PApp (PBind p A B) b). *)
-  Axiom PApp_imp : forall n a b, @ishf n a -> ~~ isabs a -> ~ P (PApp a b).
-  Axiom PProj_imp : forall  n p a, @ishf n a -> ~~ ispair a -> ~ P (PProj p a).
-  Axiom PInd_imp : forall n Q (a : PTm n) b c,
+  Axiom P_EPar : forall (a b : PTm), EPar.R a b -> P a -> P b.
+  Axiom P_RRed : forall (a b : PTm), RRed.R a b -> P a -> P b.
+  Axiom PApp_imp : forall a b, ishf a -> ~~ isabs a -> ~ P (PApp a b).
+  Axiom PProj_imp : forall p a, ishf a -> ~~ ispair a -> ~ P (PProj p a).
+  Axiom PInd_imp : forall Q (a : PTm) b c,
   ishf a ->
   ~~ iszero a ->
   ~~ issuc a  -> ~ P (PInd Q a b c).
 
-  Axiom P_AppInv : forall n (a b : PTm n), P (PApp a b) -> P a /\ P b.
-  Axiom P_AbsInv : forall n (a : PTm (S n)), P (PAbs a) -> P a.
-  Axiom P_SucInv : forall n (a : PTm n), P (PSuc a) -> P a.
-  Axiom P_BindInv : forall n p (A : PTm n) B, P (PBind p A B) -> P A /\ P B.
-  Axiom P_IndInv : forall n Q (a : PTm n) b c, P (PInd Q a b c) -> P Q /\ P a /\ P b /\ P c.
+  Axiom P_AppInv : forall (a b : PTm), P (PApp a b) -> P a /\ P b.
+  Axiom P_AbsInv : forall (a : PTm), P (PAbs a) -> P a.
+  Axiom P_SucInv : forall (a : PTm), P (PSuc a) -> P a.
+  Axiom P_BindInv : forall p (A : PTm) B, P (PBind p A B) -> P A /\ P B.
+  Axiom P_IndInv : forall Q (a : PTm) b c, P (PInd Q a b c) -> P Q /\ P a /\ P b /\ P c.
 
-  Axiom P_PairInv : forall n (a b : PTm n), P (PPair a b) -> P a /\ P b.
-  Axiom P_ProjInv : forall n p (a : PTm n), P (PProj p a) -> P a.
-  Axiom P_renaming : forall n m (ξ : fin n -> fin m) a , P (ren_PTm ξ a) <-> P a.
-
+  Axiom P_PairInv : forall (a b : PTm), P (PPair a b) -> P a /\ P b.
+  Axiom P_ProjInv : forall p (a : PTm), P (PProj p a) -> P a.
+  Axiom P_renaming : forall (ξ : nat -> nat) a , P (ren_PTm ξ a) <-> P a.
 End NoForbid.
 
 Module Type NoForbid_FactSig (M : NoForbid).
 
-  Axiom P_EPars : forall n (a b : PTm n), rtc EPar.R a b -> M.P a -> M.P b.
+  Axiom P_EPars : forall (a b : PTm), rtc EPar.R a b -> M.P a -> M.P b.
 
-  Axiom P_RReds : forall n (a b : PTm n), rtc RRed.R a b -> M.P a -> M.P b.
+  Axiom P_RReds : forall (a b : PTm), rtc RRed.R a b -> M.P a -> M.P b.
 
 End NoForbid_FactSig.
 
 Module NoForbid_Fact (M : NoForbid) : NoForbid_FactSig M.
   Import M.
 
-  Lemma P_EPars : forall n (a b : PTm n), rtc EPar.R a b -> P a -> P b.
+  Lemma P_EPars : forall (a b : PTm), rtc EPar.R a b -> P a -> P b.
   Proof.
     induction 1; eauto using P_EPar, rtc_l, rtc_refl.
   Qed.
 
-  Lemma P_RReds : forall n (a b : PTm n), rtc RRed.R a b -> P a -> P b.
+  Lemma P_RReds : forall (a b : PTm), rtc RRed.R a b -> P a -> P b.
   Proof.
     induction 1; eauto using P_RRed, rtc_l, rtc_refl.
   Qed.
@@ -1312,62 +1292,61 @@ End NoForbid_Fact.
 
 Module SN_NoForbid <: NoForbid.
   Definition P := @SN.
-  Arguments P {n}.
 
-  Lemma P_EPar : forall n (a b : PTm n), EPar.R a b -> P a -> P b.
+  Lemma P_EPar : forall (a b : PTm), EPar.R a b -> P a -> P b.
   Proof. sfirstorder use:epar_sn_preservation. Qed.
 
-  Lemma P_RRed : forall n (a b : PTm n), RRed.R a b -> P a -> P b.
+  Lemma P_RRed : forall (a b : PTm), RRed.R a b -> P a -> P b.
   Proof. hauto q:on use:red_sn_preservation, RPar.FromRRed. Qed.
 
-  Lemma PApp_imp : forall n a b, @ishf n a -> ~~ isabs a -> ~ P (PApp a b).
+  Lemma PApp_imp : forall a b, ishf a -> ~~ isabs a -> ~ P (PApp a b).
     sfirstorder use:fp_red.PApp_imp. Qed.
-  Lemma PProj_imp : forall  n p a, @ishf n a -> ~~ ispair a -> ~ P (PProj p a).
+  Lemma PProj_imp : forall p a, ishf a -> ~~ ispair a -> ~ P (PProj p a).
     sfirstorder use:fp_red.PProj_imp. Qed.
 
-  Lemma PInd_imp : forall n Q (a : PTm n) b c,
+  Lemma PInd_imp : forall Q (a : PTm) b c,
       ishf a ->
       ~~ iszero a ->
       ~~ issuc a  -> ~ P (PInd Q a b c).
   Proof. sfirstorder use: fp_red.PInd_imp. Qed.
 
-  Lemma P_AppInv : forall n (a b : PTm n), P (PApp a b) -> P a /\ P b.
+  Lemma P_AppInv : forall (a b : PTm), P (PApp a b) -> P a /\ P b.
   Proof. sfirstorder use:SN_AppInv. Qed.
 
-  Lemma P_PairInv : forall n (a b : PTm n), P (PPair a b) -> P a /\ P b.
-    move => n a b. move E : (PPair a b) => u h.
-    move : a b E. elim : n u / h; sauto lq:on rew:off. Qed.
+  Lemma P_PairInv : forall (a b : PTm), P (PPair a b) -> P a /\ P b.
+    move => a b. move E : (PPair a b) => u h.
+    move : a b E. elim : u / h; sauto lq:on rew:off. Qed.
 
-  Lemma P_ProjInv : forall n p (a : PTm n), P (PProj p a) -> P a.
+  Lemma P_ProjInv : forall p (a : PTm), P (PProj p a) -> P a.
   Proof. sfirstorder use:SN_ProjInv. Qed.
 
-  Lemma P_BindInv : forall n p (A : PTm n) B, P (PBind p A B) -> P A /\ P B.
+  Lemma P_BindInv : forall p (A : PTm) B, P (PBind p A B) -> P A /\ P B.
   Proof.
-    move => n p A B.
+    move => p A B.
     move E : (PBind p A B) => u hu.
-    move : p A B E. elim : n u /hu=>//=;sauto lq:on rew:off.
+    move : p A B E. elim : u /hu=>//=;sauto lq:on rew:off.
   Qed.
 
-  Lemma P_SucInv : forall n (a : PTm n), P (PSuc a) -> P a.
+  Lemma P_SucInv : forall (a : PTm), P (PSuc a) -> P a.
   Proof. sauto lq:on. Qed.
 
-  Lemma P_AbsInv : forall n (a : PTm (S n)), P (PAbs a) -> P a.
+  Lemma P_AbsInv : forall (a : PTm), P (PAbs a) -> P a.
   Proof.
-    move => n a. move E : (PAbs a) => u h.
+    move => a. move E : (PAbs a) => u h.
     move : E. move : a.
     induction h; sauto lq:on rew:off.
   Qed.
 
-  Lemma P_renaming : forall n m (ξ : fin n -> fin m) a , P (ren_PTm ξ a) <-> P  a.
+  Lemma P_renaming : forall (ξ : nat -> nat) a , P (ren_PTm ξ a) <-> P  a.
   Proof. hauto lq:on use:sn_antirenaming, sn_renaming. Qed.
 
-  Lemma P_ProjBind : forall n p p' (A : PTm n) B, ~ P (PProj p (PBind p' A B)).
+  Lemma P_ProjBind : forall p p' (A : PTm) B, ~ P (PProj p (PBind p' A B)).
   Proof. sfirstorder use:PProjBind_imp. Qed.
 
-  Lemma P_AppBind : forall n p (A : PTm n) B b, ~ P (PApp (PBind p A B) b).
+  Lemma P_AppBind : forall p (A : PTm) B b, ~ P (PApp (PBind p A B) b).
   Proof. sfirstorder use:PAppBind_imp. Qed.
 
-  Lemma P_IndInv : forall n Q (a : PTm n) b c, P (PInd Q a b c) -> P Q /\ P a /\ P b /\ P c.
+  Lemma P_IndInv : forall Q (a : PTm) b c, P (PInd Q a b c) -> P Q /\ P a /\ P b /\ P c.
   Proof. sfirstorder use:SN_IndInv. Qed.
 
 End SN_NoForbid.
@@ -1378,13 +1357,13 @@ Module UniqueNF (M : NoForbid) (MFacts : NoForbid_FactSig M).
   Import M MFacts.
   #[local]Hint Resolve P_EPar P_RRed PApp_imp PProj_imp : forbid.
 
-  Lemma η_split n (a0 a1 : PTm n) :
+  Lemma η_split (a0 a1 : PTm) :
     EPar.R a0 a1 ->
     P a0 ->
     exists b, rtc RRed.R a0 b /\ NeEPar.R_nonelim b a1.
   Proof.
-    move => h. elim : n a0 a1 /h .
-    - move => n a0 a1 ha ih /[dup] hP.
+    move => h. elim : a0 a1 /h .
+    - move => a0 a1 ha ih /[dup] hP.
       move /P_AbsInv /P_AppInv => [/P_renaming ha0 _].
       have {ih} := ih ha0.
       move => [b [ih0 ih1]].
@@ -1404,7 +1383,13 @@ Module UniqueNF (M : NoForbid) (MFacts : NoForbid_FactSig M).
         by eauto using RReds.renaming.
         apply rtc_refl.
         apply : RRed.AbsCong => /=.
-        apply RRed.AppAbs'. by asimpl.
+        apply RRed.AppAbs'. asimpl.
+        set y := subst_PTm _ _.
+        suff : ren_PTm id p = y. by asimpl.
+        subst y.
+        substify.
+        apply ext_PTm.
+        case => //=.
       (* violates SN *)
       + move /P_AbsInv in hP.
         have {}hP : P (PApp (ren_PTm shift b) (VarPTm var_zero))
@@ -1414,7 +1399,7 @@ Module UniqueNF (M : NoForbid) (MFacts : NoForbid_FactSig M).
         have ? : ishf (ren_PTm shift b) by scongruence use:ishf_ren.
         exfalso.
         sfirstorder use:PApp_imp.
-    - move => n a0 a1 h ih /[dup] hP.
+    - move => a0 a1 h ih /[dup] hP.
       move /P_PairInv => [/P_ProjInv + _].
       move : ih => /[apply].
       move => [b [ih0 ih1]].
@@ -1439,7 +1424,7 @@ Module UniqueNF (M : NoForbid) (MFacts : NoForbid_FactSig M).
         move : P_RReds hP. repeat move/[apply] => /=.
         sfirstorder use:PProj_imp.
     - hauto lq:on ctrs:NeEPar.R_nonelim use:RReds.AbsCong, P_AbsInv.
-    - move => n a0 a1 b0 b1 ha iha hb ihb.
+    - move => a0 a1 b0 b1 ha iha hb ihb.
       move => /[dup] hP /P_AppInv [hP0 hP1].
       have {iha} [a2 [iha0 iha1]]  := iha hP0.
       have {ihb} [b2 [ihb0 ihb1]]  := ihb hP1.
@@ -1462,7 +1447,7 @@ Module UniqueNF (M : NoForbid) (MFacts : NoForbid_FactSig M).
           have : P (PApp a2 b0) by sfirstorder use:RReds.AppCong, @rtc_refl, P_RReds.
           sfirstorder use:PApp_imp.
     - hauto lq:on ctrs:NeEPar.R_nonelim use:RReds.PairCong, P_PairInv.
-    - move => n p a0 a1 ha ih /[dup] hP /P_ProjInv.
+    - move => p a0 a1 ha ih /[dup] hP /P_ProjInv.
       move : ih => /[apply]. move => [a2 [iha0 iha1]].
       case /orP : (orNb (ishf a2)) => [h|].
       exists (PProj p a2).
@@ -1487,8 +1472,7 @@ Module UniqueNF (M : NoForbid) (MFacts : NoForbid_FactSig M).
     - hauto l:on.
     - hauto lq:on ctrs:NeEPar.R_nonelim, rtc use:RReds.BindCong, P_BindInv.
     - hauto lq:on ctrs:NeEPar.R_nonelim, rtc use:RReds.BindCong, P_BindInv.
-    - hauto l:on ctrs:NeEPar.R_nonelim.
-    - move => n P0 P1 a0 a1 b0 b1 c0 c1 hP ihP ha iha hb ihb hc ihc /[dup] hInd /P_IndInv.
+    - move => P0 P1 a0 a1 b0 b1 c0 c1 hP ihP ha iha hb ihb hc ihc /[dup] hInd /P_IndInv.
       move => []. move : ihP => /[apply].
       move => [P01][ihP0]ihP1.
       move => []. move : iha => /[apply].
@@ -1514,32 +1498,32 @@ Module UniqueNF (M : NoForbid) (MFacts : NoForbid_FactSig M).
     - hauto lq:on ctrs:NeEPar.R_nonelim use:RReds.SucCong, P_SucInv.
   Qed.
 
-  Lemma eta_postponement n a b c :
-    @P n a ->
+  Lemma eta_postponement a b c :
+    P a ->
     EPar.R a b ->
     RRed.R b c ->
     exists d, rtc RRed.R a d /\ EPar.R d c.
   Proof.
     move => + h.
     move : c.
-    elim : n a b /h => //=.
-    - move => n a0 a1 ha iha c /[dup] hP /P_AbsInv /P_AppInv [/P_renaming hP' _] hc.
+    elim : a b /h => //=.
+    - move => a0 a1 ha iha c /[dup] hP /P_AbsInv /P_AppInv [/P_renaming hP' _] hc.
       move : iha (hP') (hc); repeat move/[apply].
       move => [d [h0 h1]].
       exists  (PAbs (PApp (ren_PTm shift d) (VarPTm var_zero))).
       split. hauto lq:on rew:off ctrs:rtc use:RReds.AbsCong, RReds.AppCong, RReds.renaming.
       hauto lq:on ctrs:EPar.R.
-    - move => n a0 a1 ha iha c /P_PairInv [/P_ProjInv + _].
+    - move => a0 a1 ha iha c /P_PairInv [/P_ProjInv + _].
       move /iha => /[apply].
       move => [d [h0 h1]].
       exists (PPair (PProj PL d) (PProj PR d)).
       hauto lq:on ctrs:EPar.R use:RReds.PairCong, RReds.ProjCong.
-    - move => n a0 a1 ha iha c  /P_AbsInv /[swap].
+    - move => a0 a1 ha iha c  /P_AbsInv /[swap].
       elim /RRed.inv => //=_.
       move => a2 a3 + [? ?]. subst.
       move : iha; repeat move/[apply].
       hauto lq:on use:RReds.AbsCong ctrs:EPar.R.
-    - move => n a0 a1 b0 b1 ha iha hb ihb c hP.
+    - move => a0 a1 b0 b1 ha iha hb ihb c hP.
       elim /RRed.inv => //= _.
       + move => a2 b2 [*]. subst.
         have [hP' hP''] : P a0 /\ P b0 by sfirstorder use:P_AppInv.
@@ -1558,7 +1542,7 @@ Module UniqueNF (M : NoForbid) (MFacts : NoForbid_FactSig M).
           apply RRed.AppCong0. apply RRed.AbsCong. simpl. apply RRed.AppAbs.
           asimpl.
           apply rtc_once.
-          apply RRed.AppAbs.
+          apply RRed.AppAbs'. by asimpl.
         * exfalso.
           move : hP h0. clear => hP h0.
           have : rtc RRed.R (PApp a0 b0) (PApp (PPair (PProj PL a1) (PProj PR a1)) b0)
@@ -1569,7 +1553,7 @@ Module UniqueNF (M : NoForbid) (MFacts : NoForbid_FactSig M).
           split.
           apply : rtc_r; last by apply RRed.AppAbs.
           hauto lq:on ctrs:rtc use:RReds.AppCong.
-          hauto l:on inv:option use:EPar.morphing,NeEPar.ToEPar.
+          hauto l:on inv:nat use:EPar.morphing,NeEPar.ToEPar.
       + move => a2 a3 b2 ha2 [*]. subst.
         move : iha (ha2) {ihb} => /[apply].
         have : P a0 by sfirstorder use:P_AppInv.
@@ -1582,10 +1566,10 @@ Module UniqueNF (M : NoForbid) (MFacts : NoForbid_FactSig M).
         have : P b0 by sfirstorder use:P_AppInv.
         move : ihb hb2; repeat move /[apply].
         hauto lq:on rew:off ctrs:EPar.R, rtc use:RReds.AppCong.
-    - move => n a0 a1 b0 b1 ha iha hb ihb c /P_PairInv [hP hP'].
+    - move => a0 a1 b0 b1 ha iha hb ihb c /P_PairInv [hP hP'].
       elim /RRed.inv => //=_;
         hauto lq:on rew:off ctrs:EPar.R, rtc use:RReds.PairCong.
-    - move => n p a0 a1 ha iha c /[dup] hP /P_ProjInv hP'.
+    - move => p a0 a1 ha iha c /[dup] hP /P_ProjInv hP'.
       elim / RRed.inv => //= _.
       + move => p0 a2 b0 [*]. subst.
         move : η_split hP'  ha; repeat move/[apply].
@@ -1619,8 +1603,7 @@ Module UniqueNF (M : NoForbid) (MFacts : NoForbid_FactSig M).
     - hauto lq:on inv:RRed.R ctrs:rtc.
     - sauto lq:on ctrs:EPar.R, rtc use:RReds.BindCong, P_BindInv, @relations.rtc_transitive.
     - hauto lq:on inv:RRed.R ctrs:rtc.
-    - hauto q:on ctrs:rtc inv:RRed.R.
-    - move => n P0 P1 a0 a1 b0 b1 c0 c1 hP ihP ha iha hb ihb hc ihc u.
+    - move => P0 P1 a0 a1 b0 b1 c0 c1 hP ihP ha iha hb ihb hc ihc u.
       move => /[dup] hInd.
       move /P_IndInv.
       move => [pP0][pa0][pb0]pc0.
@@ -1650,7 +1633,12 @@ Module UniqueNF (M : NoForbid) (MFacts : NoForbid_FactSig M).
           apply : rtc_r.
           apply RReds.IndCong; eauto; eauto using rtc_refl.
           apply RRed.IndSuc.
-          apply EPar.morphing;eauto. hauto lq:on ctrs:EPar.R inv:option use:NeEPar.ToEPar.
+          apply EPar.morphing;eauto.
+          case => [|].
+          hauto lq:on rew:off ctrs:EPar.R use:NeEPar.ToEPar.
+          case => [|i].
+          hauto lq:on rew:off ctrs:EPar.R use:NeEPar.ToEPar.
+          asimpl. apply EPar.VarTm.
       + move => P2 P3 a2 b2 c hP0 [*]. subst.
         move : ihP hP0 pP0. repeat move/[apply].
         move => [P2][h0]h1.
@@ -1672,7 +1660,7 @@ Module UniqueNF (M : NoForbid) (MFacts : NoForbid_FactSig M).
         exists (PInd P0 a0 b0 c2).
         sfirstorder use:RReds.IndCong, @rtc_refl, EPar.IndCong.
     - hauto lq:on inv:RRed.R ctrs:rtc, EPar.R.
-    - move => n a0 a1 ha iha u /P_SucInv ha0.
+    - move => a0 a1 ha iha u /P_SucInv ha0.
       elim /RRed.inv => //= _ a2 a3 h [*]. subst.
       move : iha (ha0) (h); repeat move/[apply].
       move => [a2 [ih0 ih1]].
@@ -1681,8 +1669,8 @@ Module UniqueNF (M : NoForbid) (MFacts : NoForbid_FactSig M).
       by apply EPar.SucCong.
   Qed.
 
-  Lemma η_postponement_star n a b c :
-    @P n a ->
+  Lemma η_postponement_star a b c :
+    P a ->
     EPar.R a b ->
     rtc RRed.R b c ->
     exists d, rtc RRed.R a d /\ EPar.R d c.
@@ -1698,8 +1686,8 @@ Module UniqueNF (M : NoForbid) (MFacts : NoForbid_FactSig M).
       sfirstorder use:@relations.rtc_transitive.
   Qed.
 
-  Lemma η_postponement_star' n a b c :
-    @P n a ->
+  Lemma η_postponement_star' a b c :
+    P a ->
     EPar.R a b ->
     rtc RRed.R b c ->
     exists d, rtc RRed.R a d /\ NeEPar.R_nonelim d c.
@@ -1716,7 +1704,7 @@ End UniqueNF.
 Module SN_UniqueNF := UniqueNF SN_NoForbid NoForbid_FactSN.
 
 Module ERed.
-  Inductive R {n} : PTm n -> PTm n ->  Prop :=
+  Inductive R : PTm -> PTm ->  Prop :=
 
   (****************** Eta ***********************)
   | AppEta a :
@@ -1765,9 +1753,9 @@ Module ERed.
     R a0 a1 ->
     R (PSuc a0) (PSuc a1).
 
-  Derive Dependent Inversion inv with (forall n (a b : PTm n), R a b) Sort Prop.
+  Derive Inversion inv with (forall (a b : PTm), R a b) Sort Prop.
 
-  Lemma ToEPar n (a b : PTm n) :
+  Lemma ToEPar (a b : PTm) :
     ERed.R a b -> EPar.R a b.
   Proof.
     induction 1; hauto lq:on use:EPar.refl ctrs:EPar.R.
@@ -1777,38 +1765,34 @@ Module ERed.
     let x := Fresh.in_goal (Option.get (Ident.of_string "x")) in
     intro $x;
     lazy_match! Constr.type (Control.hyp x) with
-    | fin _ -> _ _ => (ltac1:(case;hauto q:on depth:2 ctrs:ERed.R))
+    | nat -> _ => (ltac1:(case;hauto q:on depth:2 ctrs:ERed.R))
     | _ => solve_anti_ren ()
     end.
 
   Ltac solve_anti_ren := ltac2:(Control.enter solve_anti_ren).
 
-  (* Definition down n m (ξ : fin n -> fin m) (a : fin (S n)) : fin m. *)
-  (*   destruct a. *)
-  (*   exact (ξ f). *)
-
-  Lemma AppEta' n a u :
-    u = (@PApp (S n) (ren_PTm shift a) (VarPTm var_zero)) ->
+  Lemma AppEta' a u :
+    u = (PApp (ren_PTm shift a) (VarPTm var_zero)) ->
     R (PAbs u) a.
   Proof. move => ->. apply AppEta. Qed.
 
-  Lemma renaming n m (a b : PTm n) (ξ : fin n -> fin m) :
+  Lemma renaming (a b : PTm) (ξ : nat -> nat) :
     R a b -> R (ren_PTm ξ a) (ren_PTm ξ b).
   Proof.
-    move => h. move : m ξ.
-    elim : n a b /h.
+    move => h. move : ξ.
+    elim : a b /h.
 
-    move => n a m ξ /=.
+    move => a ξ /=.
     apply AppEta'; eauto. by asimpl.
     all : qauto ctrs:R.
   Qed.
 
   (* Characterization of variable freeness conditions *)
-  Definition tm_i_free {n} a (i : fin n) := exists m (ξ ξ0 : fin n -> fin m), ξ i <> ξ0 i /\ ren_PTm ξ a = ren_PTm ξ0 a.
+  Definition tm_i_free a (i : fin n) := exists m (ξ ξ0 : fin n -> fin m), ξ i <> ξ0 i /\ ren_PTm a = ren_PTm0 a.
 
   Lemma subst_differ_one_ren_up n m i (ξ0 ξ1 : fin n -> fin m) :
     (forall j, i <> j -> ξ0 j = ξ1 j) ->
-    (forall j, shift i <> j -> upRen_PTm_PTm ξ0 j =  upRen_PTm_PTm ξ1 j).
+    (forall j, shift i <> j -> upRen_PTm_PTm0 j =  upRen_PTm_PTm1 j).
   Proof.
     move => hξ.
     destruct j. asimpl.
@@ -1820,7 +1804,7 @@ Module ERed.
   Lemma tm_free_ren_any n a i :
     tm_i_free a i ->
     forall m (ξ0 ξ1 : fin n -> fin m), (forall j, i <> j -> ξ0 j = ξ1 j) ->
-             ren_PTm ξ0 a = ren_PTm ξ1 a.
+             ren_PTm0 a = ren_PTm1 a.
   Proof.
     rewrite /tm_i_free.
     move => [+ [+ [+ +]]].
@@ -1841,7 +1825,7 @@ Module ERed.
       move /subst_differ_one_ren_up in hξ.
       move /(_ (shift i)) in iha.
       move : iha hξ. repeat move/[apply].
-      move /(_ _ (upRen_PTm_PTm ρ0) (upRen_PTm_PTm ρ1)).
+      move /(_ _ (upRen_PTm_PTm0) (upRen_PTm_PTm1)).
       apply. hauto l:on.
     - hauto lq:on rew:off.
     - hauto lq:on rew:off.
@@ -1851,12 +1835,12 @@ Module ERed.
     - admit.
   Admitted.
 
-  Lemma antirenaming n m (a : PTm n) (b : PTm m) (ξ : fin n -> fin m) :
+  Lemma antirenaming n m (a : PTm) (b : PTm) (ξ : fin n -> fin m) :
     (forall i j, ξ i = ξ j -> i = j) ->
-    R (ren_PTm ξ a) b -> exists b0, R a b0 /\ ren_PTm ξ b0 = b.
+    R (ren_PTm a) b -> exists b0, R a b0 /\ ren_PTm b0 = b.
   Proof.
     move => hξ.
-    move E : (ren_PTm ξ a) => u hu.
+    move E : (ren_PTm a) => u hu.
     move : n ξ a hξ E.
     elim : m u b / hu; try solve_anti_ren.
     - move => n a m ξ []//=.
@@ -1870,7 +1854,7 @@ Module ERed.
       move => [p ?]. subst.
       move : h. asimpl.
       replace (ren_PTm (funcomp shift ξ) p) with
-        (ren_PTm shift (ren_PTm ξ p)); last by asimpl.
+        (ren_PTm shift (ren_PTm p)); last by asimpl.
       move /ren_injective.
       move /(_ ltac:(hauto l:on)).
       move => ?. subst.
@@ -1886,14 +1870,14 @@ Module ERed.
       sauto lq:on use:up_injective.
     - move => n p A B0 B1 hB ihB m ξ + hξ.
       case => //= p' A2 B2 [*]. subst.
-      have : (forall i j, (upRen_PTm_PTm ξ) i = (upRen_PTm_PTm ξ) j -> i = j) by sauto.
+      have : (forall i j, (upRen_PTm_PTm) i = (upRen_PTm_PTm) j -> i = j) by sauto.
       move => {}/ihB => ihB.
       spec_refl.
       sauto lq:on.
   Admitted.
 
-  Lemma substing n m (a b : PTm n) (ρ : fin n -> PTm m) :
-    R a b -> R (subst_PTm ρ a) (subst_PTm ρ b).
+  Lemma substing n m (a b : PTm) (ρ : fin n -> PTm) :
+    R a b -> R (subst_PTm a) (subst_PTm b).
   Proof.
     move => h. move : m ρ. elim : n a b /h => n.
     move => a m ρ /=.
@@ -1901,7 +1885,7 @@ Module ERed.
     all : hauto lq:on ctrs:R.
   Qed.
 
-  Lemma nf_preservation n (a b : PTm n) :
+  Lemma nf_preservation n (a b : PTm) :
     ERed.R a b -> (nf a -> nf b) /\ (ne a -> ne b).
   Proof.
     move => h.
@@ -1925,36 +1909,36 @@ Module EReds.
     rtc ERed.R (PAbs a) (PAbs b).
   Proof. solve_s. Qed.
 
-  Lemma AppCong n (a0 a1 b0 b1 : PTm n) :
+  Lemma AppCong n (a0 a1 b0 b1 : PTm) :
     rtc ERed.R a0 a1 ->
     rtc ERed.R b0 b1 ->
     rtc ERed.R (PApp a0 b0) (PApp a1 b1).
   Proof. solve_s. Qed.
 
-  Lemma PairCong n (a0 a1 b0 b1 : PTm n) :
+  Lemma PairCong n (a0 a1 b0 b1 : PTm) :
     rtc ERed.R a0 a1 ->
     rtc ERed.R b0 b1 ->
     rtc ERed.R (PPair a0 b0) (PPair a1 b1).
   Proof. solve_s. Qed.
 
-  Lemma ProjCong n p (a0 a1  : PTm n) :
+  Lemma ProjCong n p (a0 a1  : PTm) :
     rtc ERed.R a0 a1 ->
     rtc ERed.R (PProj p a0) (PProj p a1).
   Proof. solve_s. Qed.
 
-  Lemma BindCong n p (A0 A1 : PTm n) B0 B1 :
+  Lemma BindCong n p (A0 A1 : PTm) B0 B1 :
     rtc ERed.R A0 A1 ->
     rtc ERed.R B0 B1 ->
     rtc ERed.R (PBind p A0 B0) (PBind p A1 B1).
   Proof. solve_s. Qed.
 
 
-  Lemma SucCong n (a0 a1 : PTm n) :
+  Lemma SucCong n (a0 a1 : PTm) :
     rtc ERed.R a0 a1 ->
     rtc ERed.R (PSuc a0) (PSuc a1).
   Proof. solve_s. Qed.
 
-  Lemma IndCong n P0 P1 (a0 a1 : PTm n) b0 b1 c0 c1 :
+  Lemma IndCong n P0 P1 (a0 a1 : PTm) b0 b1 c0 c1 :
     rtc ERed.R P0 P1 ->
     rtc ERed.R a0 a1 ->
     rtc ERed.R b0 b1 ->
@@ -1962,11 +1946,11 @@ Module EReds.
     rtc ERed.R (PInd P0 a0 b0 c0) (PInd P1 a1 b1 c1).
   Proof. solve_s. Qed.
 
-  Lemma renaming n m (a b : PTm n) (ξ : fin n -> fin m) :
-    rtc ERed.R a b -> rtc ERed.R (ren_PTm ξ a) (ren_PTm ξ b).
+  Lemma renaming n m (a b : PTm) (ξ : fin n -> fin m) :
+    rtc ERed.R a b -> rtc ERed.R (ren_PTm a) (ren_PTm b).
   Proof. induction 1; hauto l:on use:ERed.renaming ctrs:rtc. Qed.
 
-  Lemma FromEPar n (a b : PTm n) :
+  Lemma FromEPar n (a b : PTm) :
     EPar.R a b ->
     rtc ERed.R a b.
   Proof.
@@ -1981,18 +1965,18 @@ Module EReds.
       apply ERed.PairEta.
   Qed.
 
-  Lemma FromEPars n (a b : PTm n) :
+  Lemma FromEPars n (a b : PTm) :
     rtc EPar.R a b ->
     rtc ERed.R a b.
   Proof. induction 1; hauto l:on use:FromEPar, @relations.rtc_transitive. Qed.
 
-  Lemma substing n m (a b : PTm n) (ρ : fin n -> PTm m) :
-    rtc ERed.R a b -> rtc ERed.R (subst_PTm ρ a) (subst_PTm ρ b).
+  Lemma substing n m (a b : PTm) (ρ : fin n -> PTm) :
+    rtc ERed.R a b -> rtc ERed.R (subst_PTm a) (subst_PTm b).
   Proof.
     induction 1; hauto lq:on ctrs:rtc use:ERed.substing.
   Qed.
 
-  Lemma app_inv n (a0 b0 C : PTm n) :
+  Lemma app_inv n (a0 b0 C : PTm) :
     rtc ERed.R (PApp a0 b0) C ->
     exists a1 b1, C = PApp a1 b1 /\
                rtc ERed.R a0 a1 /\
@@ -2006,7 +1990,7 @@ Module EReds.
       hauto lq:on rew:off ctrs:rtc, ERed.R inv:ERed.R.
   Qed.
 
-  Lemma proj_inv n p (a C : PTm n) :
+  Lemma proj_inv n p (a C : PTm) :
     rtc ERed.R (PProj p a) C ->
     exists c, C = PProj p c /\ rtc ERed.R a c.
   Proof.
@@ -2016,7 +2000,7 @@ Module EReds.
       scrush ctrs:rtc,ERed.R inv:ERed.R.
   Qed.
 
-  Lemma bind_inv n p (A : PTm n) B C :
+  Lemma bind_inv n p (A : PTm) B C :
     rtc ERed.R (PBind p A B) C ->
     exists A0 B0, C = PBind p A0 B0 /\ rtc ERed.R A A0 /\ rtc ERed.R B B0.
   Proof.
@@ -2027,7 +2011,7 @@ Module EReds.
     hauto lq:on rew:off ctrs:rtc, ERed.R inv:ERed.R, rtc.
   Qed.
 
-  Lemma suc_inv n (a : PTm n) C :
+  Lemma suc_inv n (a : PTm) C :
     rtc ERed.R (PSuc a) C ->
     exists b, rtc ERed.R a b /\ C = PSuc b.
   Proof.
@@ -2038,14 +2022,14 @@ Module EReds.
     - hauto lq:on rew:off ctrs:rtc, ERed.R inv:ERed.R, rtc.
   Qed.
 
-  Lemma zero_inv n (C : PTm n) :
+  Lemma zero_inv n (C : PTm) :
     rtc ERed.R PZero C -> C = PZero.
     move E : PZero => u hu.
     move : E. elim : u C /hu=>//=.
     - hauto lq:on rew:off ctrs:rtc, ERed.R inv:ERed.R, rtc.
   Qed.
 
-  Lemma ind_inv n P (a : PTm n) b c C :
+  Lemma ind_inv n P (a : PTm) b c C :
     rtc ERed.R (PInd P a b c) C ->
     exists P0 a0 b0 c0,  rtc ERed.R P P0 /\ rtc ERed.R a a0 /\
                       rtc ERed.R b b0 /\ rtc ERed.R c c0 /\
@@ -2063,37 +2047,37 @@ End EReds.
 #[export]Hint Constructors ERed.R RRed.R EPar.R : red.
 
 Module EJoin.
-  Definition R {n} (a b : PTm n) := exists c, rtc ERed.R a c /\ rtc ERed.R b c.
+  Definition R (a b : PTm) := exists c, rtc ERed.R a c /\ rtc ERed.R b c.
 
-  Lemma hne_app_inj n (a0 b0 a1 b1 : PTm n) :
+  Lemma hne_app_inj n (a0 b0 a1 b1 : PTm) :
     R (PApp a0 b0) (PApp a1 b1) ->
     R a0 a1 /\ R b0 b1.
   Proof.
     hauto lq:on use:EReds.app_inv.
   Qed.
 
-  Lemma hne_proj_inj n p0 p1 (a0 a1 : PTm n) :
+  Lemma hne_proj_inj n p0 p1 (a0 a1 : PTm) :
     R (PProj p0 a0) (PProj p1 a1) ->
     p0 = p1 /\ R a0 a1.
   Proof.
     hauto lq:on rew:off use:EReds.proj_inv.
   Qed.
 
-  Lemma bind_inj n p0 p1 (A0 A1 : PTm n) B0 B1 :
+  Lemma bind_inj n p0 p1 (A0 A1 : PTm) B0 B1 :
     R (PBind p0 A0 B0) (PBind p1 A1 B1) ->
     p0 = p1 /\ R A0 A1 /\ R B0 B1.
   Proof.
     hauto lq:on rew:off use:EReds.bind_inv.
   Qed.
 
-  Lemma suc_inj n  (A0 A1 : PTm n)  :
+  Lemma suc_inj n  (A0 A1 : PTm)  :
     R (PSuc A0) (PSuc A1) ->
     R A0 A1.
   Proof.
     hauto lq:on rew:off use:EReds.suc_inv.
   Qed.
 
-  Lemma ind_inj n P0 P1 (a0 a1 : PTm n) b0 b1 c0 c1 :
+  Lemma ind_inj n P0 P1 (a0 a1 : PTm) b0 b1 c0 c1 :
     R (PInd P0 a0 b0 c0) (PInd P1 a1 b1 c1) ->
     R P0 P1 /\ R a0 a1 /\ R b0 b1 /\ R c0 c1.
   Proof. hauto q:on use:EReds.ind_inv. Qed.
@@ -2101,7 +2085,7 @@ Module EJoin.
 End EJoin.
 
 Module RERed.
-  Inductive R {n} : PTm n -> PTm n ->  Prop :=
+  Inductive R : PTm -> PTm ->  Prop :=
   (****************** Beta ***********************)
   | AppAbs a b :
     R (PApp (PAbs a) b)  (subst_PTm (scons b VarPTm) a)
@@ -2162,79 +2146,79 @@ Module RERed.
     R a0 a1 ->
     R (PSuc a0) (PSuc a1).
 
-  Lemma ToBetaEta n (a b : PTm n) :
+  Lemma ToBetaEta n (a b : PTm) :
     R a b ->
     ERed.R a b \/ RRed.R a b.
   Proof. induction 1; hauto lq:on db:red. Qed.
 
-  Lemma FromBeta n (a b : PTm n) :
+  Lemma FromBeta n (a b : PTm) :
     RRed.R a b -> RERed.R a b.
   Proof. induction 1; qauto l:on ctrs:R. Qed.
 
-  Lemma FromEta n (a b : PTm n) :
+  Lemma FromEta n (a b : PTm) :
     ERed.R a b -> RERed.R a b.
   Proof. induction 1; qauto l:on ctrs:R. Qed.
 
-  Lemma ToBetaEtaPar n (a b : PTm n) :
+  Lemma ToBetaEtaPar n (a b : PTm) :
     R a b ->
     EPar.R a b \/ RRed.R a b.
   Proof.
     hauto q:on use:ERed.ToEPar, ToBetaEta.
   Qed.
 
-  Lemma sn_preservation n (a b : PTm n) :
+  Lemma sn_preservation n (a b : PTm) :
     R a b ->
     SN a ->
     SN b.
   Proof. hauto q:on use:ToBetaEtaPar, epar_sn_preservation, red_sn_preservation, RPar.FromRRed. Qed.
 
-  Lemma bind_preservation n (a b : PTm n) :
+  Lemma bind_preservation n (a b : PTm) :
     R a b -> isbind a -> isbind b.
   Proof. hauto q:on inv:R. Qed.
 
-  Lemma univ_preservation n (a b : PTm n) :
+  Lemma univ_preservation n (a b : PTm) :
     R a b -> isuniv a -> isuniv b.
   Proof. hauto q:on inv:R. Qed.
 
-  Lemma nat_preservation n (a b : PTm n) :
+  Lemma nat_preservation n (a b : PTm) :
     R a b -> isnat a -> isnat b.
   Proof. hauto q:on inv:R. Qed.
 
-  Lemma sne_preservation n (a b : PTm n) :
+  Lemma sne_preservation n (a b : PTm) :
     R a b -> SNe a -> SNe b.
   Proof.
     hauto q:on use:ToBetaEtaPar, RPar.FromRRed use:red_sn_preservation, epar_sn_preservation.
   Qed.
 
-  Lemma substing n m (a b : PTm n) (ρ : fin n -> PTm m) :
-    RERed.R a b -> RERed.R (subst_PTm ρ a) (subst_PTm ρ b).
+  Lemma substing n m (a b : PTm) (ρ : fin n -> PTm) :
+    RERed.R a b -> RERed.R (subst_PTm a) (subst_PTm b).
   Proof.
     hauto q:on use:ToBetaEta, FromBeta, FromEta, RRed.substing, ERed.substing.
   Qed.
 
-  Lemma hne_preservation n (a b : PTm n) :
+  Lemma hne_preservation n (a b : PTm) :
     RERed.R a b -> ishne a -> ishne b.
   Proof.  induction 1; sfirstorder. Qed.
 
 End RERed.
 
 Module REReds.
-  Lemma hne_preservation n (a b : PTm n) :
+  Lemma hne_preservation n (a b : PTm) :
     rtc RERed.R a b -> ishne a -> ishne b.
   Proof.  induction 1; eauto using RERed.hne_preservation, rtc_refl, rtc. Qed.
 
-  Lemma sn_preservation n (a b : PTm n) :
+  Lemma sn_preservation n (a b : PTm) :
     rtc RERed.R a b ->
     SN a ->
     SN b.
   Proof. induction 1; eauto using RERed.sn_preservation. Qed.
 
-  Lemma FromRReds n (a b : PTm n) :
+  Lemma FromRReds n (a b : PTm) :
     rtc RRed.R a b ->
     rtc RERed.R a b.
   Proof. induction 1; hauto lq:on ctrs:rtc use:RERed.FromBeta. Qed.
 
-  Lemma FromEReds n (a b : PTm n) :
+  Lemma FromEReds n (a b : PTm) :
     rtc ERed.R a b ->
     rtc RERed.R a b.
   Proof. induction 1; hauto lq:on ctrs:rtc use:RERed.FromEta. Qed.
@@ -2251,29 +2235,29 @@ Module REReds.
     rtc RERed.R (PAbs a) (PAbs b).
   Proof. solve_s. Qed.
 
-  Lemma AppCong n (a0 a1 b0 b1 : PTm n) :
+  Lemma AppCong n (a0 a1 b0 b1 : PTm) :
     rtc RERed.R a0 a1 ->
     rtc RERed.R b0 b1 ->
     rtc RERed.R (PApp a0 b0) (PApp a1 b1).
   Proof. solve_s. Qed.
 
-  Lemma PairCong n (a0 a1 b0 b1 : PTm n) :
+  Lemma PairCong n (a0 a1 b0 b1 : PTm) :
     rtc RERed.R a0 a1 ->
     rtc RERed.R b0 b1 ->
     rtc RERed.R (PPair a0 b0) (PPair a1 b1).
   Proof. solve_s. Qed.
 
-  Lemma ProjCong n p (a0 a1  : PTm n) :
+  Lemma ProjCong n p (a0 a1  : PTm) :
     rtc RERed.R a0 a1 ->
     rtc RERed.R (PProj p a0) (PProj p a1).
   Proof. solve_s. Qed.
 
-  Lemma SucCong n (a0 a1 : PTm n) :
+  Lemma SucCong n (a0 a1 : PTm) :
     rtc RERed.R a0 a1 ->
     rtc RERed.R (PSuc a0) (PSuc a1).
   Proof. solve_s. Qed.
 
-  Lemma IndCong n P0 P1 (a0 a1 : PTm n) b0 b1 c0 c1 :
+  Lemma IndCong n P0 P1 (a0 a1 : PTm) b0 b1 c0 c1 :
     rtc RERed.R P0 P1 ->
     rtc RERed.R a0 a1 ->
     rtc RERed.R b0 b1 ->
@@ -2281,25 +2265,25 @@ Module REReds.
     rtc RERed.R (PInd P0 a0 b0 c0) (PInd P1 a1 b1 c1).
   Proof. solve_s. Qed.
 
-  Lemma BindCong n p (A0 A1 : PTm n) B0 B1 :
+  Lemma BindCong n p (A0 A1 : PTm) B0 B1 :
     rtc RERed.R A0 A1 ->
     rtc RERed.R B0 B1 ->
     rtc RERed.R (PBind p A0 B0) (PBind p A1 B1).
   Proof. solve_s. Qed.
 
-  Lemma bind_preservation n (a b : PTm n) :
+  Lemma bind_preservation n (a b : PTm) :
     rtc RERed.R a b -> isbind a -> isbind b.
   Proof. induction 1; qauto l:on ctrs:rtc use:RERed.bind_preservation. Qed.
 
-  Lemma univ_preservation n (a b : PTm n) :
+  Lemma univ_preservation n (a b : PTm) :
     rtc RERed.R a b -> isuniv a -> isuniv b.
   Proof. induction 1; qauto l:on ctrs:rtc use:RERed.univ_preservation. Qed.
 
-  Lemma nat_preservation n (a b : PTm n) :
+  Lemma nat_preservation n (a b : PTm) :
     rtc RERed.R a b -> isnat a -> isnat b.
   Proof. induction 1; qauto l:on ctrs:rtc use:RERed.nat_preservation. Qed.
 
-  Lemma sne_preservation n (a b : PTm n) :
+  Lemma sne_preservation n (a b : PTm) :
     rtc RERed.R a b -> SNe a -> SNe b.
   Proof. induction 1; qauto l:on ctrs:rtc use:RERed.sne_preservation. Qed.
 
@@ -2329,7 +2313,7 @@ Module REReds.
     move : i E. elim : u C /hu; hauto lq:on rew:off inv:RERed.R.
   Qed.
 
-  Lemma hne_app_inv n (a0 b0 C : PTm n) :
+  Lemma hne_app_inv n (a0 b0 C : PTm) :
     rtc RERed.R (PApp a0 b0) C ->
     ishne a0 ->
     exists a1 b1, C = PApp a1 b1 /\
@@ -2344,7 +2328,7 @@ Module REReds.
       hauto lq:on rew:off ctrs:rtc, RERed.R use:RERed.hne_preservation inv:RERed.R.
   Qed.
 
-  Lemma hne_proj_inv n p (a C : PTm n) :
+  Lemma hne_proj_inv n p (a C : PTm) :
     rtc RERed.R (PProj p a) C ->
     ishne a ->
     exists c, C = PProj p c /\ rtc RERed.R a c.
@@ -2355,7 +2339,7 @@ Module REReds.
       scrush ctrs:rtc,RERed.R use:RERed.hne_preservation inv:RERed.R.
   Qed.
 
-  Lemma hne_ind_inv n P a b c (C : PTm n) :
+  Lemma hne_ind_inv n P a b c (C : PTm) :
     rtc RERed.R (PInd P a b c) C -> ishne a ->
     exists P0 a0 b0 c0, C = PInd P0 a0 b0 c0 /\
                      rtc RERed.R P P0 /\
@@ -2369,47 +2353,47 @@ Module REReds.
       scrush ctrs:rtc,RERed.R use:RERed.hne_preservation inv:RERed.R.
   Qed.
 
-  Lemma substing n m (a b : PTm n) (ρ : fin n -> PTm m) :
-    rtc RERed.R a b -> rtc RERed.R (subst_PTm ρ a) (subst_PTm ρ b).
+  Lemma substing n m (a b : PTm) (ρ : fin n -> PTm) :
+    rtc RERed.R a b -> rtc RERed.R (subst_PTm a) (subst_PTm b).
   Proof.
     induction 1; hauto lq:on ctrs:rtc use:RERed.substing.
   Qed.
 
 
-  Lemma cong_up n m (ρ0 ρ1 : fin n -> PTm m) :
+  Lemma cong_up n m (ρ0 ρ1 : fin n -> PTm) :
     (forall i, rtc RERed.R (ρ0 i) (ρ1 i)) ->
-    (forall i, rtc RERed.R (up_PTm_PTm ρ0 i) (up_PTm_PTm ρ1 i)).
+    (forall i, rtc RERed.R (up_PTm_PTm0 i) (up_PTm_PTm1 i)).
   Proof. move => h i. destruct i as [i|].
          simpl. rewrite /funcomp.
          substify. by apply substing.
          apply rtc_refl.
   Qed.
 
-  Lemma cong_up2 n m (ρ0 ρ1 : fin n -> PTm m) :
+  Lemma cong_up2 n m (ρ0 ρ1 : fin n -> PTm) :
     (forall i, rtc RERed.R (ρ0 i) (ρ1 i)) ->
-    (forall i, rtc RERed.R (up_PTm_PTm (up_PTm_PTm ρ0) i) (up_PTm_PTm (up_PTm_PTm ρ1) i)).
+    (forall i, rtc RERed.R (up_PTm_PTm (up_PTm_PTm0) i) (up_PTm_PTm (up_PTm_PTm1) i)).
   Proof. hauto l:on use:cong_up. Qed.
 
-  Lemma cong n m (a : PTm n) (ρ0 ρ1 : fin n -> PTm m) :
+  Lemma cong n m (a : PTm) (ρ0 ρ1 : fin n -> PTm) :
     (forall i, rtc RERed.R (ρ0 i) (ρ1 i)) ->
-    rtc RERed.R (subst_PTm ρ0 a) (subst_PTm ρ1 a).
+    rtc RERed.R (subst_PTm0 a) (subst_PTm1 a).
   Proof.
     move : m ρ0 ρ1. elim : n / a => /=;
       eauto 20 using AppCong, AbsCong, BindCong, ProjCong, PairCong, cong_up, rtc_refl, IndCong, SucCong, cong_up2.
   Qed.
 
-  Lemma cong' n m (a b : PTm n) (ρ0 ρ1 : fin n -> PTm m) :
+  Lemma cong' n m (a b : PTm) (ρ0 ρ1 : fin n -> PTm) :
     rtc RERed.R a b ->
     (forall i, rtc RERed.R (ρ0 i) (ρ1 i)) ->
-    rtc RERed.R (subst_PTm ρ0 a) (subst_PTm ρ1 b).
+    rtc RERed.R (subst_PTm0 a) (subst_PTm1 b).
   Proof.
     move => h0 h1.
-    have : rtc RERed.R (subst_PTm ρ0 a) (subst_PTm ρ1 a) by eauto using cong.
+    have : rtc RERed.R (subst_PTm0 a) (subst_PTm1 a) by eauto using cong.
     move => ?. apply : relations.rtc_transitive; eauto.
     hauto l:on use:substing.
   Qed.
 
-  Lemma ToEReds n (a b : PTm n) :
+  Lemma ToEReds n (a b : PTm) :
     nf a ->
     rtc RERed.R a b -> rtc ERed.R a b.
   Proof.
@@ -2417,14 +2401,14 @@ Module REReds.
     induction h; hauto lq:on rew:off ctrs:rtc use:RERed.ToBetaEta, RReds.nf_refl, @rtc_once, ERed.nf_preservation.
   Qed.
 
-  Lemma zero_inv n (C : PTm n) :
+  Lemma zero_inv n (C : PTm) :
     rtc RERed.R PZero C -> C = PZero.
     move E : PZero => u hu.
     move : E. elim : u C /hu=>//=.
     - hauto lq:on rew:off ctrs:rtc, RERed.R inv:RERed.R, rtc.
   Qed.
 
-  Lemma suc_inv n (a : PTm n) C :
+  Lemma suc_inv n (a : PTm) C :
     rtc RERed.R (PSuc a) C ->
     exists b, rtc RERed.R a b /\ C = PSuc b.
   Proof.
@@ -2447,7 +2431,7 @@ Module REReds.
 End REReds.
 
 Module LoRed.
-  Inductive R {n} : PTm n -> PTm n ->  Prop :=
+  Inductive R : PTm -> PTm ->  Prop :=
   (****************** Beta ***********************)
   | AppAbs a b :
     R (PApp (PAbs a) b)  (subst_PTm (scons b VarPTm) a)
@@ -2515,7 +2499,7 @@ Module LoRed.
     R a0 a1 ->
     R (PSuc a0) (PSuc a1).
 
-  Lemma hf_preservation n (a b : PTm n) :
+  Lemma hf_preservation n (a b : PTm) :
     LoRed.R a b ->
     ishf a ->
     ishf b.
@@ -2523,12 +2507,12 @@ Module LoRed.
     move => h. elim : n a b /h=>//=.
   Qed.
 
-  Lemma ToRRed n (a b : PTm n) :
+  Lemma ToRRed n (a b : PTm) :
     LoRed.R a b ->
     RRed.R a b.
   Proof. induction 1; hauto lq:on ctrs:RRed.R. Qed.
 
-  Lemma AppAbs' n a (b : PTm n) u :
+  Lemma AppAbs' n a (b : PTm) u :
     u = (subst_PTm (scons b VarPTm) a) ->
     R (PApp (PAbs a) b)  u.
   Proof. move => ->. apply AppAbs. Qed.
@@ -2538,8 +2522,8 @@ Module LoRed.
     R (@PInd n P (PSuc a) b c) u.
   Proof. move => ->. apply IndSuc. Qed.
 
-  Lemma renaming n m (a b : PTm n) (ξ : fin n -> fin m) :
-    R a b -> R (ren_PTm ξ a) (ren_PTm ξ b).
+  Lemma renaming n m (a b : PTm) (ξ : fin n -> fin m) :
+    R a b -> R (ren_PTm a) (ren_PTm b).
   Proof.
     move => h. move : m ξ.
     elim : n a b /h.
@@ -2553,7 +2537,7 @@ Module LoRed.
 End LoRed.
 
 Module LoReds.
-  Lemma hf_preservation n (a b : PTm n) :
+  Lemma hf_preservation n (a b : PTm) :
     rtc LoRed.R a b ->
     ishf a ->
     ishf b.
@@ -2561,7 +2545,7 @@ Module LoReds.
     induction 1; eauto using LoRed.hf_preservation.
   Qed.
 
-  Lemma hf_ne_imp n (a b : PTm n) :
+  Lemma hf_ne_imp n (a b : PTm) :
     rtc LoRed.R a b ->
     ne b ->
     ~~ ishf a.
@@ -2582,34 +2566,34 @@ Module LoReds.
     rtc LoRed.R (PAbs a) (PAbs b).
   Proof. solve_s. Qed.
 
-  Lemma AppCong n (a0 a1 b0 b1 : PTm n) :
+  Lemma AppCong n (a0 a1 b0 b1 : PTm) :
     rtc LoRed.R a0 a1 ->
     rtc LoRed.R b0 b1 ->
     ne a1 ->
     rtc LoRed.R (PApp a0 b0) (PApp a1 b1).
   Proof. solve_s. Qed.
 
-  Lemma PairCong n (a0 a1 b0 b1 : PTm n) :
+  Lemma PairCong n (a0 a1 b0 b1 : PTm) :
     rtc LoRed.R a0 a1 ->
     rtc LoRed.R b0 b1 ->
     nf a1 ->
     rtc LoRed.R (PPair a0 b0) (PPair a1 b1).
   Proof. solve_s. Qed.
 
-  Lemma ProjCong n p (a0 a1  : PTm n) :
+  Lemma ProjCong n p (a0 a1  : PTm) :
     rtc LoRed.R a0 a1 ->
     ne a1 ->
     rtc LoRed.R (PProj p a0) (PProj p a1).
   Proof. solve_s. Qed.
 
-  Lemma BindCong n p (A0 A1 : PTm n) B0 B1 :
+  Lemma BindCong n p (A0 A1 : PTm) B0 B1 :
     rtc LoRed.R A0 A1 ->
     rtc LoRed.R B0 B1 ->
     nf A1 ->
     rtc LoRed.R (PBind p A0 B0) (PBind p A1 B1).
   Proof. solve_s. Qed.
 
-  Lemma IndCong n P0 P1 (a0 a1 : PTm n) b0 b1 c0 c1 :
+  Lemma IndCong n P0 P1 (a0 a1 : PTm) b0 b1 c0 c1 :
     rtc LoRed.R a0 a1 ->
     rtc LoRed.R P0 P1 ->
     rtc LoRed.R b0 b1 ->
@@ -2620,7 +2604,7 @@ Module LoReds.
     rtc LoRed.R (PInd P0 a0 b0 c0) (PInd P1 a1 b1 c1).
   Proof. solve_s. Qed.
 
-  Lemma SucCong n (a0 a1 : PTm n) :
+  Lemma SucCong n (a0 a1 : PTm) :
     rtc LoRed.R a0 a1 ->
     rtc LoRed.R (PSuc a0) (PSuc a1).
   Proof. solve_s. Qed.
@@ -2628,9 +2612,9 @@ Module LoReds.
   Local Ltac triv := simpl in *; itauto.
 
   Lemma FromSN_mutual : forall n,
-    (forall (a : PTm n) (_ : SNe a), exists v, rtc LoRed.R a v /\ ne v) /\
-    (forall (a : PTm n) (_ : SN a), exists v, rtc LoRed.R a v /\ nf v) /\
-    (forall (a b : PTm n) (_ : TRedSN a b), LoRed.R a b).
+    (forall (a : PTm) (_ : SNe a), exists v, rtc LoRed.R a v /\ ne v) /\
+    (forall (a : PTm) (_ : SN a), exists v, rtc LoRed.R a v /\ nf v) /\
+    (forall (a b : PTm) (_ : TRedSN a b), LoRed.R a b).
   Proof.
     apply sn_mutual.
     - hauto lq:on ctrs:rtc.
@@ -2666,49 +2650,49 @@ Module LoReds.
   Lemma FromSN : forall n a, @SN n a -> exists v, rtc LoRed.R a v /\ nf v.
   Proof. firstorder using FromSN_mutual. Qed.
 
-  Lemma ToRReds : forall n (a b : PTm n), rtc LoRed.R a b -> rtc RRed.R a b.
+  Lemma ToRReds : forall n (a b : PTm), rtc LoRed.R a b -> rtc RRed.R a b.
   Proof. induction 1; hauto lq:on ctrs:rtc use:LoRed.ToRRed. Qed.
 
 End LoReds.
 
 
-Fixpoint size_PTm {n} (a : PTm n) :=
+Fixpoint size_PTm (a : PTm) :=
   match a with
   | VarPTm _ => 1
-  | PAbs a => 3 + size_PTm a
-  | PApp a b => 1 + Nat.add (size_PTm a) (size_PTm b)
-  | PProj p a => 1 + size_PTm a
-  | PPair a b => 3 + Nat.add (size_PTm a) (size_PTm b)
+  | PAbs a => 3 + size_PTm
+  | PApp a b => 1 + Nat.add (size_PTm) (size_PTm)
+  | PProj p a => 1 + size_PTm
+  | PPair a b => 3 + Nat.add (size_PTm) (size_PTm)
   | PUniv _ => 3
-  | PBind p A B => 3 + Nat.add (size_PTm A) (size_PTm B)
-  | PInd P a b c => 3 + size_PTm P + size_PTm a + size_PTm b + size_PTm c
+  | PBind p A B => 3 + Nat.add (size_PTm) (size_PTm)
+  | PInd P a b c => 3 + size_PTm + size_PTm + size_PTm + size_PTm
   | PNat => 3
-  | PSuc a => 3 + size_PTm a
+  | PSuc a => 3 + size_PTm
   | PZero => 3
   | PBot => 1
   end.
 
-Lemma size_PTm_ren n m (ξ : fin n -> fin m) a : size_PTm (ren_PTm ξ a) = size_PTm a.
+Lemma size_PTm_ren n m (ξ : fin n -> fin m) a : size_PTm (ren_PTm a) = size_PTm.
 Proof.
   move : m ξ. elim : n / a => //=; scongruence.
 Qed.
 
 #[export]Hint Rewrite size_PTm_ren : sizetm.
 
-Lemma ered_size {n} (a b : PTm n) :
+Lemma ered_size (a b : PTm) :
   ERed.R a b ->
-  size_PTm b < size_PTm a.
+  size_PTm < size_PTm.
 Proof.
   move => h. elim : n a b /h; hauto l:on rew:db:sizetm.
 Qed.
 
-Lemma ered_sn n (a : PTm n) : sn ERed.R a.
+Lemma ered_sn n (a : PTm) : sn ERed.R a.
 Proof.
   hauto lq:on rew:off use:size_PTm_ren, ered_size,
           well_founded_lt_compat unfold:well_founded.
 Qed.
 
-Lemma ered_local_confluence n (a b c : PTm n) :
+Lemma ered_local_confluence n (a b c : PTm) :
   ERed.R a b ->
   ERed.R a c ->
   exists d, rtc ERed.R b d  /\ rtc ERed.R c d.
@@ -2814,7 +2798,7 @@ Proof.
   - qauto l:on inv:ERed.R ctrs:rtc use:EReds.SucCong.
 Qed.
 
-Lemma ered_confluence n (a b c : PTm n) :
+Lemma ered_confluence n (a b c : PTm) :
   rtc ERed.R a b ->
   rtc ERed.R a c ->
   exists d, rtc ERed.R b d  /\ rtc ERed.R c d.
@@ -2822,18 +2806,18 @@ Proof.
   sfirstorder use:relations.locally_confluent_confluent, ered_sn, ered_local_confluence.
 Qed.
 
-Lemma red_confluence n (a b c : PTm n) :
+Lemma red_confluence n (a b c : PTm) :
   rtc RRed.R a b ->
   rtc RRed.R a c ->
   exists d, rtc RRed.R b d  /\ rtc RRed.R c d.
-  suff : rtc RPar.R a b -> rtc RPar.R a c -> exists d : PTm n, rtc RPar.R b d /\ rtc RPar.R c d
+  suff : rtc RPar.R a b -> rtc RPar.R a c -> exists d : PTm, rtc RPar.R b d /\ rtc RPar.R c d
              by hauto lq:on use:RReds.RParIff.
   apply relations.diamond_confluent.
   rewrite /relations.diamond.
   eauto using RPar.diamond.
 Qed.
 
-Lemma red_uniquenf n (a b c : PTm n) :
+Lemma red_uniquenf n (a b c : PTm) :
   rtc RRed.R a b ->
   rtc RRed.R a c ->
   nf b ->
@@ -2848,20 +2832,20 @@ Proof.
 Qed.
 
 Module NeEPars.
-  Lemma R_nonelim_nf n (a b : PTm n) :
+  Lemma R_nonelim_nf n (a b : PTm) :
     rtc NeEPar.R_nonelim a b ->
     nf b ->
     nf a.
   Proof. induction 1; sfirstorder use:NeEPar.R_elim_nf. Qed.
 
-  Lemma ToEReds : forall n, (forall (a b : PTm n), rtc NeEPar.R_nonelim a b -> rtc ERed.R a b).
+  Lemma ToEReds : forall n, (forall (a b : PTm), rtc NeEPar.R_nonelim a b -> rtc ERed.R a b).
   Proof.
     induction 1; hauto l:on use:NeEPar.ToEPar, EReds.FromEPar, @relations.rtc_transitive.
   Qed.
 End NeEPars.
 
 
-Lemma rered_standardization n (a c : PTm n) :
+Lemma rered_standardization n (a c : PTm) :
   SN a ->
   rtc RERed.R a c ->
   exists b, rtc RRed.R a b /\ rtc NeEPar.R_nonelim b c.
@@ -2878,7 +2862,7 @@ Proof.
   - hauto lq:on ctrs:rtc use:red_sn_preservation, RPar.FromRRed.
 Qed.
 
-Lemma rered_confluence n (a b c : PTm n) :
+Lemma rered_confluence n (a b c : PTm) :
   SN a ->
   rtc RERed.R a b ->
   rtc RERed.R a c ->
@@ -2912,14 +2896,14 @@ Qed.
 
 (* Beta joinability *)
 Module BJoin.
-  Definition R {n} (a b : PTm n) := exists c, rtc RRed.R a c /\ rtc RRed.R b c.
-  Lemma refl n (a : PTm n) : R a a.
+  Definition R (a b : PTm) := exists c, rtc RRed.R a c /\ rtc RRed.R b c.
+  Lemma refl n (a : PTm) : R a a.
   Proof. sfirstorder use:@rtc_refl unfold:R. Qed.
 
-  Lemma symmetric n (a b : PTm n) : R a b -> R b a.
+  Lemma symmetric n (a b : PTm) : R a b -> R b a.
   Proof. sfirstorder unfold:R. Qed.
 
-  Lemma transitive n (a b c : PTm n) : R a b -> R b c -> R a c.
+  Lemma transitive n (a b c : PTm) : R a b -> R b c -> R a c.
   Proof.
     rewrite /R.
     move => [ab [ha +]] [bc [+ hc]].
@@ -2933,7 +2917,7 @@ Module BJoin.
   (*   R (PAbs a) (PAbs b). *)
   (* Proof. hauto lq:on use:RReds.AbsCong unfold:R. Qed. *)
 
-  (* Lemma AppCong n (a0 a1 b0 b1 : PTm n) : *)
+  (* Lemma AppCong n (a0 a1 b0 b1 : PTm) : *)
   (*   R a0 a1 -> *)
   (*   R b0 b1 -> *)
   (*   R (PApp a0 b0) (PApp a1 b1). *)
@@ -2941,21 +2925,21 @@ Module BJoin.
 End BJoin.
 
 Module DJoin.
-  Definition R {n} (a b : PTm n) := exists c, rtc RERed.R a c /\ rtc RERed.R b c.
+  Definition R (a b : PTm) := exists c, rtc RERed.R a c /\ rtc RERed.R b c.
 
-  Lemma refl n (a : PTm n) : R a a.
+  Lemma refl n (a : PTm) : R a a.
   Proof. sfirstorder use:@rtc_refl unfold:R. Qed.
 
-  Lemma FromEJoin n (a b : PTm n) : EJoin.R a b -> DJoin.R a b.
+  Lemma FromEJoin n (a b : PTm) : EJoin.R a b -> DJoin.R a b.
   Proof. hauto q:on use:REReds.FromEReds. Qed.
 
-  Lemma ToEJoin n (a b : PTm n) : nf a -> nf b -> DJoin.R a b -> EJoin.R a b.
+  Lemma ToEJoin n (a b : PTm) : nf a -> nf b -> DJoin.R a b -> EJoin.R a b.
   Proof. hauto q:on use:REReds.ToEReds. Qed.
 
-  Lemma symmetric n (a b : PTm n) : R a b -> R b a.
+  Lemma symmetric n (a b : PTm) : R a b -> R b a.
   Proof. sfirstorder unfold:R. Qed.
 
-  Lemma transitive n (a b c : PTm n) : SN b -> R a b -> R b c -> R a c.
+  Lemma transitive n (a b c : PTm) : SN b -> R a b -> R b c -> R a c.
   Proof.
     rewrite /R.
     move => + [ab [ha +]] [bc [+ hc]].
@@ -2969,30 +2953,30 @@ Module DJoin.
     R (PAbs a) (PAbs b).
   Proof. hauto lq:on use:REReds.AbsCong unfold:R. Qed.
 
-  Lemma AppCong n (a0 a1 b0 b1 : PTm n) :
+  Lemma AppCong n (a0 a1 b0 b1 : PTm) :
     R a0 a1 ->
     R b0 b1 ->
     R (PApp a0 b0) (PApp a1 b1).
   Proof. hauto lq:on use:REReds.AppCong unfold:R. Qed.
 
-  Lemma PairCong n (a0 a1 b0 b1 : PTm n) :
+  Lemma PairCong n (a0 a1 b0 b1 : PTm) :
     R a0 a1 ->
     R b0 b1 ->
     R (PPair a0 b0) (PPair a1 b1).
   Proof. hauto q:on use:REReds.PairCong. Qed.
 
-  Lemma ProjCong n p (a0 a1  : PTm n) :
+  Lemma ProjCong n p (a0 a1  : PTm) :
     R a0 a1 ->
     R (PProj p a0) (PProj p a1).
   Proof. hauto q:on use:REReds.ProjCong. Qed.
 
-  Lemma BindCong n p (A0 A1 : PTm n) B0 B1 :
+  Lemma BindCong n p (A0 A1 : PTm) B0 B1 :
     R A0 A1 ->
     R B0 B1 ->
     R (PBind p A0 B0) (PBind p A1 B1).
   Proof. hauto q:on use:REReds.BindCong. Qed.
 
-  Lemma IndCong n P0 P1 (a0 a1 : PTm n) b0 b1 c0 c1 :
+  Lemma IndCong n P0 P1 (a0 a1 : PTm) b0 b1 c0 c1 :
     R P0 P1 ->
     R a0 a1 ->
     R b0 b1 ->
@@ -3000,12 +2984,12 @@ Module DJoin.
     R (PInd P0 a0 b0 c0) (PInd P1 a1 b1 c1).
   Proof. hauto q:on use:REReds.IndCong. Qed.
 
-  Lemma SucCong n (a0 a1 : PTm n) :
+  Lemma SucCong n (a0 a1 : PTm) :
     R a0 a1 ->
     R (PSuc a0) (PSuc a1).
   Proof. qauto l:on use:REReds.SucCong. Qed.
 
-  Lemma FromRedSNs n (a b : PTm n) :
+  Lemma FromRedSNs n (a b : PTm) :
     rtc TRedSN a b ->
     R a b.
   Proof.
@@ -3013,7 +2997,7 @@ Module DJoin.
     sfirstorder use:@rtc_refl unfold:R.
   Qed.
 
-  Lemma sne_nat_noconf n (a b : PTm n) :
+  Lemma sne_nat_noconf n (a b : PTm) :
     R a b -> SNe a -> isnat b -> False.
   Proof.
     move => [c [? ?]] *.
@@ -3021,7 +3005,7 @@ Module DJoin.
     qauto l:on inv:SNe.
   Qed.
 
-  Lemma sne_bind_noconf n (a b : PTm n) :
+  Lemma sne_bind_noconf n (a b : PTm) :
     R a b -> SNe a -> isbind b -> False.
   Proof.
     move => [c [? ?]] *.
@@ -3029,14 +3013,14 @@ Module DJoin.
     qauto l:on inv:SNe.
   Qed.
 
-  Lemma sne_univ_noconf n (a b : PTm n) :
+  Lemma sne_univ_noconf n (a b : PTm) :
     R a b -> SNe a -> isuniv b -> False.
   Proof.
     hauto q:on use:REReds.sne_preservation,
           REReds.univ_preservation inv:SNe.
   Qed.
 
-  Lemma bind_univ_noconf n (a b : PTm n) :
+  Lemma bind_univ_noconf n (a b : PTm) :
     R a b -> isbind a -> isuniv b -> False.
   Proof.
     move => [c [h0 h1]] h2 h3.
@@ -3046,7 +3030,7 @@ Module DJoin.
     case : c => //=; itauto.
   Qed.
 
-  Lemma hne_univ_noconf n (a b : PTm n) :
+  Lemma hne_univ_noconf n (a b : PTm) :
     R a b -> ishne a -> isuniv b -> False.
   Proof.
     move => [c [h0 h1]] h2 h3.
@@ -3057,7 +3041,7 @@ Module DJoin.
     case : c => //=.
   Qed.
 
-  Lemma hne_bind_noconf n (a b : PTm n) :
+  Lemma hne_bind_noconf n (a b : PTm) :
     R a b -> ishne a -> isbind b -> False.
   Proof.
     move => [c [h0 h1]] h2 h3.
@@ -3068,7 +3052,7 @@ Module DJoin.
     case : c => //=.
   Qed.
 
-  Lemma hne_nat_noconf n (a b : PTm n) :
+  Lemma hne_nat_noconf n (a b : PTm) :
     R a b -> ishne a -> isnat b -> False.
   Proof.
     move => [c [h0 h1]] h2 h3.
@@ -3076,7 +3060,7 @@ Module DJoin.
     clear. case : c => //=; itauto.
   Qed.
 
-  Lemma bind_inj n p0 p1 (A0 A1 : PTm n) B0 B1 :
+  Lemma bind_inj n p0 p1 (A0 A1 : PTm) B0 B1 :
     DJoin.R (PBind p0 A0 B0) (PBind p1 A1 B1) ->
     p0 = p1 /\ DJoin.R A0 A1 /\ DJoin.R B0 B1.
   Proof.
@@ -3094,14 +3078,14 @@ Module DJoin.
     sauto lq:on rew:off use:REReds.univ_inv.
   Qed.
 
-  Lemma suc_inj n  (A0 A1 : PTm n)  :
+  Lemma suc_inj n  (A0 A1 : PTm)  :
     R (PSuc A0) (PSuc A1) ->
     R A0 A1.
   Proof.
     hauto lq:on rew:off use:REReds.suc_inv.
   Qed.
 
-  Lemma hne_app_inj n (a0 b0 a1 b1 : PTm n) :
+  Lemma hne_app_inj n (a0 b0 a1 b1 : PTm) :
     R (PApp a0 b0) (PApp a1 b1) ->
     ishne a0 ->
     ishne a1 ->
@@ -3110,7 +3094,7 @@ Module DJoin.
     hauto lq:on use:REReds.hne_app_inv.
   Qed.
 
-  Lemma hne_proj_inj n p0 p1 (a0 a1 : PTm n) :
+  Lemma hne_proj_inj n p0 p1 (a0 a1 : PTm) :
     R (PProj p0 a0) (PProj p1 a1) ->
     ishne a0 ->
     ishne a1 ->
@@ -3119,45 +3103,45 @@ Module DJoin.
     sauto lq:on use:REReds.hne_proj_inv.
   Qed.
 
-  Lemma FromRRed0 n (a b : PTm n) :
+  Lemma FromRRed0 n (a b : PTm) :
     RRed.R a b -> R a b.
   Proof.
     hauto lq:on ctrs:rtc use:RERed.FromBeta unfold:R.
   Qed.
 
-  Lemma FromRRed1 n (a b : PTm n) :
+  Lemma FromRRed1 n (a b : PTm) :
     RRed.R b a -> R a b.
   Proof.
     hauto lq:on ctrs:rtc use:RERed.FromBeta unfold:R.
   Qed.
 
-  Lemma FromRReds n (a b : PTm n) :
+  Lemma FromRReds n (a b : PTm) :
     rtc RRed.R b a -> R a b.
   Proof.
     hauto lq:on ctrs:rtc use:REReds.FromRReds unfold:R.
   Qed.
 
-  Lemma FromBJoin n (a b : PTm n) :
+  Lemma FromBJoin n (a b : PTm) :
     BJoin.R a b -> R a b.
   Proof.
     hauto lq:on ctrs:rtc use:REReds.FromRReds unfold:R.
   Qed.
 
-  Lemma substing n m (a b : PTm n) (ρ : fin n -> PTm m) :
-    R a b -> R (subst_PTm ρ a) (subst_PTm ρ b).
+  Lemma substing n m (a b : PTm) (ρ : fin n -> PTm) :
+    R a b -> R (subst_PTm a) (subst_PTm b).
   Proof.
     hauto lq:on rew:off ctrs:rtc unfold:R use:REReds.substing.
   Qed.
 
-  Lemma renaming n m (a b : PTm n) (ρ : fin n -> fin m) :
-    R a b -> R (ren_PTm ρ a) (ren_PTm ρ b).
+  Lemma renaming n m (a b : PTm) (ρ : fin n -> fin m) :
+    R a b -> R (ren_PTm a) (ren_PTm b).
   Proof. substify. apply substing. Qed.
 
-  Lemma weakening n (a b : PTm n)  :
+  Lemma weakening n (a b : PTm)  :
     R a b -> R (ren_PTm shift a) (ren_PTm shift b).
   Proof. apply renaming. Qed.
 
-  Lemma cong n m (a : PTm (S n)) c d (ρ : fin n -> PTm m) :
+  Lemma cong n m (a : PTm (S n)) c d (ρ : fin n -> PTm) :
     R c d -> R (subst_PTm (scons c ρ) a) (subst_PTm (scons d ρ) a).
   Proof.
     rewrite /R. move => [cd [h0 h1]].
@@ -3165,7 +3149,7 @@ Module DJoin.
     hauto q:on ctrs:rtc inv:option use:REReds.cong.
   Qed.
 
-  Lemma cong' n m (a b : PTm (S n)) c d (ρ : fin n -> PTm m) :
+  Lemma cong' n m (a b : PTm (S n)) c d (ρ : fin n -> PTm) :
     R a b ->
     R c d -> R (subst_PTm (scons c ρ) a) (subst_PTm (scons d ρ) b).
   Proof.
@@ -3174,7 +3158,7 @@ Module DJoin.
     hauto q:on ctrs:rtc inv:option use:REReds.cong'.
   Qed.
 
-  Lemma pair_inj n (a0 a1 b0 b1 : PTm n) :
+  Lemma pair_inj n (a0 a1 b0 b1 : PTm) :
     SN (PPair a0 b0) ->
     SN (PPair a1 b1) ->
     R (PPair a0 b0) (PPair a1 b1) ->
@@ -3201,7 +3185,7 @@ Module DJoin.
     split; eauto using transitive.
   Qed.
 
-  Lemma ejoin_pair_inj n (a0 a1 b0 b1 : PTm n) :
+  Lemma ejoin_pair_inj n (a0 a1 b0 b1 : PTm) :
     nf a0 -> nf b0 -> nf a1 -> nf b1 ->
     EJoin.R (PPair a0 b0) (PPair a1 b1) ->
     EJoin.R a0 a1 /\ EJoin.R b0 b1.
@@ -3250,7 +3234,7 @@ Module DJoin.
     hauto l:on use:ToEJoin.
   Qed.
 
-  Lemma standardization n (a b : PTm n) :
+  Lemma standardization n (a b : PTm) :
     SN a -> SN b -> R a b ->
     exists va vb, rtc RRed.R a va /\ rtc RRed.R b vb /\ nf va /\ nf vb /\ EJoin.R va vb.
   Proof.
@@ -3270,7 +3254,7 @@ Module DJoin.
     hauto q:on use:NeEPars.ToEReds unfold:EJoin.R.
   Qed.
 
-  Lemma standardization_lo n (a b : PTm n) :
+  Lemma standardization_lo n (a b : PTm) :
     SN a -> SN b -> R a b ->
     exists va vb, rtc LoRed.R a va /\ rtc LoRed.R b vb /\ nf va /\ nf vb /\ EJoin.R va vb.
   Proof.
@@ -3288,7 +3272,7 @@ End DJoin.
 
 
 Module Sub1.
-  Inductive R {n} : PTm n -> PTm n -> Prop :=
+  Inductive R : PTm -> PTm -> Prop :=
   | Refl a :
     R a a
   | Univ i j :
@@ -3303,21 +3287,21 @@ Module Sub1.
     R B0 B1 ->
     R (PBind PSig A0 B0) (PBind PSig A1 B1).
 
-  Lemma transitive0 n (A B C : PTm n) :
+  Lemma transitive0 n (A B C : PTm) :
     R A B -> (R B C -> R A C) /\ (R C A -> R C B).
   Proof.
     move => h. move : C.
     elim : n A B /h; hauto lq:on ctrs:R inv:R solve+:lia.
   Qed.
 
-  Lemma transitive n (A B C : PTm n) :
+  Lemma transitive n (A B C : PTm) :
     R A B -> R B C -> R A C.
   Proof. hauto q:on use:transitive0. Qed.
 
-  Lemma refl n (A : PTm n) : R A A.
+  Lemma refl n (A : PTm) : R A A.
   Proof. sfirstorder. Qed.
 
-  Lemma commutativity0 n (A B C : PTm n) :
+  Lemma commutativity0 n (A B C : PTm) :
     R A B ->
     (RERed.R A C ->
     exists D, RERed.R B D /\ R C D) /\
@@ -3328,7 +3312,7 @@ Module Sub1.
     elim : n A B / h; hauto lq:on ctrs:RERed.R, R inv:RERed.R.
   Qed.
 
-  Lemma commutativity_Ls n (A B C : PTm n) :
+  Lemma commutativity_Ls n (A B C : PTm) :
     R A B ->
     rtc RERed.R A C ->
     exists D, rtc RERed.R B D /\ R C D.
@@ -3336,7 +3320,7 @@ Module Sub1.
     move => + h. move : B. induction h; sauto lq:on use:commutativity0.
   Qed.
 
-  Lemma commutativity_Rs n (A B C : PTm n) :
+  Lemma commutativity_Rs n (A B C : PTm) :
     R A B ->
     rtc RERed.R B C ->
     exists D, rtc RERed.R A D /\ R D C.
@@ -3345,46 +3329,46 @@ Module Sub1.
   Qed.
 
   Lemma sn_preservation  : forall n,
-  (forall (a : PTm n) (s : SNe a), forall b, R a b \/ R b a -> a = b) /\
-  (forall (a : PTm n) (s : SN a), forall b, R a b \/ R b a -> SN b) /\
-  (forall (a b : PTm n) (_ : TRedSN a b), forall c, R a c \/ R c a -> a = c).
+  (forall (a : PTm) (s : SNe a), forall b, R a b \/ R b a -> a = b) /\
+  (forall (a : PTm) (s : SN a), forall b, R a b \/ R b a -> SN b) /\
+  (forall (a b : PTm) (_ : TRedSN a b), forall c, R a c \/ R c a -> a = c).
   Proof.
     apply sn_mutual; hauto lq:on inv:R ctrs:SN.
   Qed.
 
-  Lemma bind_preservation n (a b : PTm n) :
+  Lemma bind_preservation n (a b : PTm) :
     R a b -> isbind a = isbind b.
   Proof. hauto q:on inv:R. Qed.
 
-  Lemma univ_preservation n (a b : PTm n) :
+  Lemma univ_preservation n (a b : PTm) :
     R a b -> isuniv a = isuniv b.
   Proof. hauto q:on inv:R. Qed.
 
-  Lemma sne_preservation n (a b : PTm n) :
+  Lemma sne_preservation n (a b : PTm) :
     R a b -> SNe a <-> SNe b.
   Proof. hfcrush use:sn_preservation. Qed.
 
-  Lemma renaming n m (a b : PTm n) (ξ : fin n -> fin m) :
-    R a b -> R (ren_PTm ξ a) (ren_PTm ξ b).
+  Lemma renaming n m (a b : PTm) (ξ : fin n -> fin m) :
+    R a b -> R (ren_PTm a) (ren_PTm b).
   Proof.
     move => h. move : m ξ.
     elim : n a b /h; hauto lq:on ctrs:R.
   Qed.
 
-  Lemma substing n m (a b : PTm n) (ρ : fin n -> PTm m) :
-    R a b -> R (subst_PTm ρ a) (subst_PTm ρ b).
+  Lemma substing n m (a b : PTm) (ρ : fin n -> PTm) :
+    R a b -> R (subst_PTm a) (subst_PTm b).
   Proof. move => h. move : m ρ. elim : n a b /h; hauto lq:on ctrs:R. Qed.
 
-  Lemma hne_refl n (a b : PTm n) :
+  Lemma hne_refl n (a b : PTm) :
     ishne a \/ ishne b -> R a b -> a = b.
   Proof. hauto q:on inv:R. Qed.
 
 End Sub1.
 
 Module ESub.
-  Definition R {n} (a b : PTm n) := exists c0 c1, rtc ERed.R a c0 /\ rtc ERed.R b c1 /\ Sub1.R c0 c1.
+  Definition R (a b : PTm) := exists c0 c1, rtc ERed.R a c0 /\ rtc ERed.R b c1 /\ Sub1.R c0 c1.
 
-  Lemma pi_inj n (A0 A1 : PTm n) B0 B1 :
+  Lemma pi_inj n (A0 A1 : PTm) B0 B1 :
     R (PBind PPi A0 B0) (PBind PPi A1 B1) ->
     R A1 A0 /\ R B0 B1.
   Proof.
@@ -3394,7 +3378,7 @@ Module ESub.
     sauto lq:on rew:off inv:Sub1.R.
   Qed.
 
-  Lemma sig_inj n (A0 A1 : PTm n) B0 B1 :
+  Lemma sig_inj n (A0 A1 : PTm) B0 B1 :
     R (PBind PSig A0 B0) (PBind PSig A1 B1) ->
     R A0 A1 /\ R B0 B1.
   Proof.
@@ -3404,7 +3388,7 @@ Module ESub.
     sauto lq:on rew:off inv:Sub1.R.
   Qed.
 
-  Lemma suc_inj n (a b : PTm n) :
+  Lemma suc_inj n (a b : PTm) :
     R (PSuc a) (PSuc b) ->
     R a b.
   Proof.
@@ -3414,12 +3398,12 @@ Module ESub.
 End ESub.
 
 Module Sub.
-  Definition R {n} (a b : PTm n) := exists c d, rtc RERed.R a c /\ rtc RERed.R b d /\ Sub1.R c d.
+  Definition R (a b : PTm) := exists c d, rtc RERed.R a c /\ rtc RERed.R b d /\ Sub1.R c d.
 
-  Lemma refl n (a : PTm n) : R a a.
+  Lemma refl n (a : PTm) : R a a.
   Proof. sfirstorder use:@rtc_refl unfold:R. Qed.
 
-  Lemma ToJoin n (a b : PTm n) :
+  Lemma ToJoin n (a b : PTm) :
     ishne a \/ ishne b ->
     R a b ->
     DJoin.R a b.
@@ -3429,7 +3413,7 @@ Module Sub.
     hauto lq:on rew:off use:Sub1.hne_refl.
   Qed.
 
-  Lemma transitive n (a b c : PTm n) : SN b -> R a b -> R b c -> R a c.
+  Lemma transitive n (a b c : PTm) : SN b -> R a b -> R b c -> R a c.
   Proof.
     rewrite /R.
     move => h  [a0][b0][ha][hb]ha0b0 [b1][c0][hb'][hc]hb1c0.
@@ -3441,10 +3425,10 @@ Module Sub.
     exists a',c'; hauto l:on use:Sub1.transitive, @relations.rtc_transitive.
   Qed.
 
-  Lemma FromJoin n (a b : PTm n) : DJoin.R a b -> R a b.
+  Lemma FromJoin n (a b : PTm) : DJoin.R a b -> R a b.
   Proof. sfirstorder. Qed.
 
-  Lemma PiCong n (A0 A1 : PTm n) B0 B1 :
+  Lemma PiCong n (A0 A1 : PTm) B0 B1 :
     R A1 A0 ->
     R B0 B1 ->
     R (PBind PPi A0 B0) (PBind PPi A1 B1).
@@ -3456,7 +3440,7 @@ Module Sub.
     repeat split; eauto using REReds.BindCong, Sub1.PiCong.
   Qed.
 
-  Lemma SigCong n (A0 A1 : PTm n) B0 B1 :
+  Lemma SigCong n (A0 A1 : PTm) B0 B1 :
     R A0 A1 ->
     R B0 B1 ->
     R (PBind PSig A0 B0) (PBind PSig A1 B1).
@@ -3473,7 +3457,7 @@ Module Sub.
     @R n (PUniv i) (PUniv j).
   Proof. hauto lq:on ctrs:Sub1.R, rtc. Qed.
 
-  Lemma sne_nat_noconf n (a b : PTm n) :
+  Lemma sne_nat_noconf n (a b : PTm) :
     R a b -> SNe a -> isnat b -> False.
   Proof.
     move => [c [d [h0 [h1 h2]]]] *.
@@ -3481,7 +3465,7 @@ Module Sub.
     move : h2. clear. hauto q:on inv:Sub1.R, SNe.
   Qed.
 
-  Lemma nat_sne_noconf n (a b : PTm n) :
+  Lemma nat_sne_noconf n (a b : PTm) :
     R a b -> isnat a -> SNe b -> False.
   Proof.
     move => [c [d [h0 [h1 h2]]]] *.
@@ -3489,7 +3473,7 @@ Module Sub.
     move : h2. clear. hauto q:on inv:Sub1.R, SNe.
   Qed.
 
-  Lemma sne_bind_noconf n (a b : PTm n) :
+  Lemma sne_bind_noconf n (a b : PTm) :
     R a b -> SNe a -> isbind b -> False.
   Proof.
     rewrite /R.
@@ -3499,7 +3483,7 @@ Module Sub.
     qauto l:on inv:SNe.
   Qed.
 
-  Lemma hne_bind_noconf n (a b : PTm n) :
+  Lemma hne_bind_noconf n (a b : PTm) :
     R a b -> ishne a -> isbind b -> False.
   Proof.
     rewrite /R.
@@ -3510,7 +3494,7 @@ Module Sub.
     clear. case : d => //=.
   Qed.
 
-  Lemma bind_sne_noconf n (a b : PTm n) :
+  Lemma bind_sne_noconf n (a b : PTm) :
     R a b -> SNe b -> isbind a -> False.
   Proof.
     rewrite /R.
@@ -3520,14 +3504,14 @@ Module Sub.
     qauto l:on inv:SNe.
   Qed.
 
-  Lemma sne_univ_noconf n (a b : PTm n) :
+  Lemma sne_univ_noconf n (a b : PTm) :
     R a b -> SNe a -> isuniv b -> False.
   Proof.
     hauto l:on use:REReds.sne_preservation,
           REReds.univ_preservation, Sub1.sne_preservation, Sub1.univ_preservation inv:SNe.
   Qed.
 
-  Lemma univ_sne_noconf n (a b : PTm n) :
+  Lemma univ_sne_noconf n (a b : PTm) :
     R a b -> SNe b -> isuniv a -> False.
   Proof.
     move => [c[d] [? []]] *.
@@ -3537,7 +3521,7 @@ Module Sub.
     clear. case : c => //=. inversion 2.
   Qed.
 
-  Lemma univ_nat_noconf n (a b : PTm n)  :
+  Lemma univ_nat_noconf n (a b : PTm)  :
     R a b -> isuniv b -> isnat a -> False.
   Proof.
     move => [c[d] [? []]] h0 h1 h2 h3.
@@ -3547,7 +3531,7 @@ Module Sub.
     clear. case : d => //=.
   Qed.
 
-  Lemma nat_univ_noconf n (a b : PTm n)  :
+  Lemma nat_univ_noconf n (a b : PTm)  :
     R a b -> isnat b -> isuniv a -> False.
   Proof.
     move => [c[d] [? []]] h0 h1 h2 h3.
@@ -3557,7 +3541,7 @@ Module Sub.
     clear. case : d => //=.
   Qed.
 
-  Lemma bind_nat_noconf n (a b : PTm n)  :
+  Lemma bind_nat_noconf n (a b : PTm)  :
     R a b -> isbind b -> isnat a -> False.
   Proof.
     move => [c[d] [? []]] h0 h1 h2 h3.
@@ -3568,7 +3552,7 @@ Module Sub.
     case : d h1 => //=.
   Qed.
 
-  Lemma nat_bind_noconf n (a b : PTm n)  :
+  Lemma nat_bind_noconf n (a b : PTm)  :
     R a b -> isnat b -> isbind a -> False.
   Proof.
     move => [c[d] [? []]] h0 h1 h2 h3.
@@ -3579,7 +3563,7 @@ Module Sub.
     case : d h1 => //=.
   Qed.
 
-  Lemma bind_univ_noconf n (a b : PTm n) :
+  Lemma bind_univ_noconf n (a b : PTm) :
     R a b -> isbind a -> isuniv b -> False.
   Proof.
     move => [c[d] [h0 [h1 h1']]] h2 h3.
@@ -3590,7 +3574,7 @@ Module Sub.
     case : c => //=; itauto.
   Qed.
 
-  Lemma univ_bind_noconf n (a b : PTm n) :
+  Lemma univ_bind_noconf n (a b : PTm) :
     R a b -> isbind b -> isuniv a -> False.
   Proof.
     move => [c[d] [h0 [h1 h1']]] h2 h3.
@@ -3601,7 +3585,7 @@ Module Sub.
     case : c => //=; itauto.
   Qed.
 
-  Lemma bind_inj n p0 p1 (A0 A1 : PTm n) B0 B1 :
+  Lemma bind_inj n p0 p1 (A0 A1 : PTm) B0 B1 :
     R (PBind p0 A0 B0) (PBind p1 A1 B1) ->
     p0 = p1 /\ (if p0 is PPi then R A1 A0 else R A0 A1) /\ R B0 B1.
   Proof.
@@ -3618,7 +3602,7 @@ Module Sub.
     sauto lq:on rew:off use:REReds.univ_inv.
   Qed.
 
-  Lemma suc_inj n  (A0 A1 : PTm n)  :
+  Lemma suc_inj n  (A0 A1 : PTm)  :
     R (PSuc A0) (PSuc A1) ->
     R A0 A1.
   Proof.
@@ -3626,7 +3610,7 @@ Module Sub.
   Qed.
 
 
-  Lemma cong n m (a b : PTm (S n)) c d (ρ : fin n -> PTm m) :
+  Lemma cong n m (a b : PTm (S n)) c d (ρ : fin n -> PTm) :
     R a b -> DJoin.R c d -> R (subst_PTm (scons c ρ) a) (subst_PTm (scons d ρ) b).
   Proof.
     rewrite /R.
@@ -3639,18 +3623,18 @@ Module Sub.
     eauto using Sub1.substing.
   Qed.
 
-  Lemma substing n m (a b : PTm n) (ρ : fin n -> PTm m) :
-    R a b -> R (subst_PTm ρ a) (subst_PTm ρ b).
+  Lemma substing n m (a b : PTm) (ρ : fin n -> PTm) :
+    R a b -> R (subst_PTm a) (subst_PTm b).
   Proof.
     rewrite /R.
     move => [a0][b0][h0][h1]h2.
     hauto ctrs:rtc use:REReds.cong', Sub1.substing.
   Qed.
 
-  Lemma ToESub n (a b : PTm n) : nf a -> nf b -> R a b -> ESub.R a b.
+  Lemma ToESub n (a b : PTm) : nf a -> nf b -> R a b -> ESub.R a b.
   Proof. hauto q:on use:REReds.ToEReds. Qed.
 
-  Lemma standardization n (a b : PTm n) :
+  Lemma standardization n (a b : PTm) :
     SN a -> SN b -> R a b ->
     exists va vb, rtc RRed.R a va /\ rtc RRed.R b vb /\ nf va /\ nf vb /\ ESub.R va vb.
   Proof.
@@ -3668,7 +3652,7 @@ Module Sub.
     hauto lq:on.
   Qed.
 
-  Lemma standardization_lo n (a b : PTm n) :
+  Lemma standardization_lo n (a b : PTm) :
     SN a -> SN b -> R a b ->
     exists va vb, rtc LoRed.R a va /\ rtc LoRed.R b vb /\ nf va /\ nf vb /\ ESub.R va vb.
   Proof.
